combine_conditions qed

Semantics/TermRewrites.thy
@@ -1,5 +1,5 @@
 theory TermRewrites
-  imports Semantics.IRTreeEvalThms Semantics.TreeToGraphThms
+  imports Semantics.IRTreeEvalThms Semantics.TreeToGraphThms Snippets.Snipping
 begin
 
 (*
@@ -268,6 +268,7 @@ Nested expressions are replaced with a string placeholder.
 
 This restricts match primitives to match just one node.
 \<close>
+snipbegin \<open>PatterExpr\<close>
 type_synonym VarName = "String.literal"
 type_synonym Vars = "VarName fset"
 
@@ -278,6 +279,7 @@ datatype PatternExpr =
   | VariablePattern VarName
   | ConstantPattern Value
   | ConstantVarPattern VarName
+snipend -
 
 
 subsection \<open>Variable Generation\<close>
@@ -336,6 +338,8 @@ datatype SideCondition =
   UpMaskEquals IRExpr "64 word" |
   DownMaskEquals IRExpr "64 word" |
   UpMaskCancels IRExpr IRExpr |
+  IsBool IRExpr |
+  PowerOf2 IRExpr |
   Empty |
   And SideCondition SideCondition |
   Not SideCondition
@@ -350,6 +354,8 @@ fun eval_condition :: "SideCondition \<Rightarrow> bool" where
   "eval_condition (UpMaskEquals e m) = (IRExpr_up e = m)" |
   "eval_condition (DownMaskEquals e m) = (IRExpr_down e = m)" |
   "eval_condition (UpMaskCancels e1 e2) = (((and (IRExpr_up e1) (IRExpr_up e2)) = 0))" |
+  "eval_condition (PowerOf2 e) = False" |
+  "eval_condition (IsBool e) = ((e = ConstantExpr (IntVal 32 0)) | (e = ConstantExpr (IntVal 32 0)))" |
   
   "eval_condition (Empty) = True" |
 
@@ -358,14 +364,14 @@ fun eval_condition :: "SideCondition \<Rightarrow> bool" where
 
 
 subsection \<open>Match Primitives\<close>
+snipbegin \<open>MATCH\<close>
 datatype MATCH =
   match VarName PatternExpr |
   equality VarName VarName (infixl "==" 52) |
   andthen MATCH MATCH (infixl "&&" 50) |
-  either MATCH MATCH (infixl "||" 49) |
-  negate SideCondition |
-  check SideCondition |
+  condition SideCondition |
   noop
+snipend -
 
 text \<open>The definitions of la and ra help to feed the scope through when generating a match pattern.\<close>
 definition la :: "('b \<Rightarrow> 'a) \<Rightarrow> (Scope \<Rightarrow> Scope \<times> 'b) \<Rightarrow> (Scope \<Rightarrow> Scope \<times> 'a)"
@@ -393,6 +399,7 @@ abbreviation descend where
 fun register_name where
   "register_name (s, m) vn v = (s, m(vn\<mapsto>v))"
 
+snipbegin "matchpattern"
 fun match_pattern :: "IRExpr \<Rightarrow> VarName \<Rightarrow> Scope \<Rightarrow> Scope \<times> MATCH" where
   "match_pattern (UnaryExpr op e) v =
     match v \<langle>
@@ -418,11 +425,14 @@ fun match_pattern :: "IRExpr \<Rightarrow> VarName \<Rightarrow> Scope \<Rightar
     (\<lambda>s. (s, match v (ConstantPattern c)))" |
   "match_pattern (ConstantVar c) v =
     (\<lambda>s. (s, match v (ConstantVarPattern c)))"
-
+snipend -
 
 subsubsection \<open>Match Primitive Semantics\<close>
+snipbegin \<open>Subst\<close>
 type_synonym Subst = "VarName \<Rightarrow> IRExpr option"
+snipend -
 
+snipbegin \<open>evalmatch\<close>
 fun eval_match :: "MATCH \<Rightarrow> Subst \<Rightarrow> Subst option" where
   "eval_match (match v (UnaryPattern op1 x)) s =
     (case s v of 
@@ -434,14 +444,14 @@ fun eval_match :: "MATCH \<Rightarrow> Subst \<Rightarrow> Subst option" where
     (case s v of
       Some (BinaryExpr op2 xe ye) \<Rightarrow>
         (if op1 = op2 
-          then Some (s(x\<mapsto>xe) ++ s(y\<mapsto>ye))
+          then Some (s(x\<mapsto>xe, y\<mapsto>ye))
           else None) |
       Some _ \<Rightarrow> None |
       None \<Rightarrow> None)" |
   "eval_match (match v (ConditionalPattern c tb fb)) s =
     (case s v of
       Some (ConditionalExpr ce te fe) \<Rightarrow>
-        (Some (s(c\<mapsto>ce) ++ s(tb\<mapsto>te) ++ s(fb\<mapsto>fe))) |
+        (Some (s(c\<mapsto>ce, tb\<mapsto>te, fb\<mapsto>fe))) |
       Some _ \<Rightarrow> None |
       None \<Rightarrow> None)" |
   "eval_match (match v (ConstantPattern c1)) s =
@@ -456,55 +466,57 @@ fun eval_match :: "MATCH \<Rightarrow> Subst \<Rightarrow> Subst option" where
       (case eval_match m1 s of 
         None \<Rightarrow> None |
         Some s' \<Rightarrow> eval_match m2 s')" |
-  "eval_match (either m1 m2) s =
-      (case eval_match m1 s of
-        None \<Rightarrow> eval_match m2 s |
-        Some s' \<Rightarrow> Some s')" |
   "eval_match noop s = Some s" |
-  "eval_match (check sc) s = Some s" | (* TODO: Check always passes *)
-  "eval_match (negate sc) s = Some s" | (* TODO: Check always passes *)
+  "eval_match (condition sc) s = (if eval_condition sc then Some s else None)" |
   "eval_match _ s = None"
-
+snipend -
 
 subsection \<open>Combining Rules\<close>
 
+snipbegin \<open>Rules\<close>
 datatype Rules =
   base IRExpr |
   cond MATCH Rules (infixl "?" 52) |
   else Rules Rules (infixl "else" 50) |
   seq Rules Rules (infixl "\<then>" 49) |
   choice "Rules list"
+snipend -
 
 text \<open>Use the scope of a generated match to replace real variable names with aliases in the rewrite result.\<close>
-fun expr_result :: "IRExpr \<Rightarrow> Scope \<Rightarrow> IRExpr" where
-  "expr_result (UnaryExpr op e) s = 
-    UnaryExpr op (expr_result e s)" |
-  "expr_result (BinaryExpr op e1 e2) s = 
-    BinaryExpr op (expr_result e1 s) (expr_result e2 s)" |
-  "expr_result (ConditionalExpr b e1 e2) s = 
-    ConditionalExpr (expr_result b s) (expr_result e1 s) (expr_result e2 s)" |
-  "expr_result (VariableExpr vn st) (s, m) = 
+snipbegin \<open>groundresult\<close>
+fun ground_result :: "IRExpr \<Rightarrow> Scope \<Rightarrow> IRExpr" where
+  "ground_result (UnaryExpr op e) s = 
+    UnaryExpr op (ground_result e s)" |
+  "ground_result (BinaryExpr op e1 e2) s = 
+    BinaryExpr op (ground_result e1 s) (ground_result e2 s)" |
+  "ground_result (ConditionalExpr b e1 e2) s = 
+    ConditionalExpr (ground_result b s) (ground_result e1 s) (ground_result e2 s)" |
+  "ground_result (VariableExpr vn st) (s, m) = 
     (case m vn of None \<Rightarrow> VariableExpr vn st 
                 | Some v' \<Rightarrow> VariableExpr v' st)" |
-  "expr_result e v = e"
+  "ground_result e v = e"
+snipend -
 
 fun ground_condition :: "SideCondition \<Rightarrow> Scope \<Rightarrow> SideCondition" where
-  "ground_condition (IsConstantExpr p) s = (IsConstantExpr (expr_result p s))" |
+  "ground_condition (IsConstantExpr p) s = (IsConstantExpr (ground_result p s))" |
   "ground_condition (WellFormed st) s = (WellFormed st)" |
-  "ground_condition (IsStamp e st) s = (IsStamp (expr_result e s) st)" |
-  "ground_condition (StampUnder e1 e2) s = (StampUnder (expr_result e1 s) (expr_result e2 s))" |
-  "ground_condition (UpMaskEquals e m) s = (UpMaskEquals (expr_result e s) m)" |
-  "ground_condition (DownMaskEquals e m) s = (DownMaskEquals (expr_result e s) m)" |
-  "ground_condition (UpMaskCancels e1 e2) s = (UpMaskCancels (expr_result e1 s) (expr_result e2 s))" |
+  "ground_condition (IsStamp e st) s = (IsStamp (ground_result e s) st)" |
+  "ground_condition (StampUnder e1 e2) s = (StampUnder (ground_result e1 s) (ground_result e2 s))" |
+  "ground_condition (UpMaskEquals e m) s = (UpMaskEquals (ground_result e s) m)" |
+  "ground_condition (DownMaskEquals e m) s = (DownMaskEquals (ground_result e s) m)" |
+  "ground_condition (UpMaskCancels e1 e2) s = (UpMaskCancels (ground_result e1 s) (ground_result e2 s))" |
+  "ground_condition (PowerOf2 e) s = (PowerOf2 (ground_result e s))" |
+  "ground_condition (IsBool e) s = (IsBool (ground_result e s))" |
   "ground_condition (And sc1 sc2) s = And (ground_condition sc1 s) (ground_condition sc2 s)" |
   "ground_condition (Not sc) s = Not (ground_condition sc s)" |
   "ground_condition (Empty) s = Empty"
 
+snipbegin \<open>generate\<close>
 fun generate :: "IRExpr \<Rightarrow> IRExpr \<Rightarrow> SideCondition \<Rightarrow> Rules" where
   "generate p r sc = 
     (let (s, m) = match_pattern p STR ''e'' ({||}, (\<lambda>x. None))
-     in ((m && check (ground_condition sc s)) ? (base (expr_result r s))))"
-
+     in ((m && condition (ground_condition sc s)) ? (base (ground_result r s))))"
+snipend -
 
 subsubsection \<open>Rules Semantics\<close>
 definition start_unification where
@@ -565,6 +577,22 @@ inductive eval_rules :: "Rules \<Rightarrow> Subst \<Rightarrow> IRExpr option \
   "\<lbrakk>eval_rules r1 u None;
     eval_rules r2 u r\<rbrakk>
    \<Longrightarrow> eval_rules (r1 \<then> r2) u r"
+
+declare [[show_types=false,show_sorts=false]]
+snipbegin \<open>rules-semantics\<close>
+text \<open>
+\induct{@{thm[mode=Rule] eval_rules.intros(1) [no_vars]}}{evalrules:base}
+\induct{@{thm[mode=Rule] eval_rules.intros(2) [no_vars]}}{evalrules:cond-some}
+\induct{@{thm[mode=Rule] eval_rules.intros(3) [no_vars]}}{evalrules:cond-none}
+\induct{@{thm[mode=Rule] eval_rules.intros(4) [no_vars]}}{evalrules:else-some}
+\induct{@{thm[mode=Rule] eval_rules.intros(5) [no_vars]}}{evalrules:else-none}
+\induct{@{thm[mode=Rule] eval_rules.intros(6) [no_vars]}}{evalrules:choice-some}
+\induct{@{thm[mode=Rule] eval_rules.intros(7) [no_vars]}}{evalrules:choice-none}
+\induct{@{thm[mode=Rule] eval_rules.intros(8) [no_vars]}}{evalrules:choice-empty}
+\induct{@{thm[mode=Rule] eval_rules.intros(9) [no_vars]}}{evalrules:seq-some}
+\induct{@{thm[mode=Rule] eval_rules.intros(10) [no_vars]}}{evalrules:seq-none}
+\<close>
+snipend -
 
 inductive_cases baseE: "eval_rules (base e') u e"
 inductive_cases condE: "eval_rules (cond m r) u e"
@@ -635,9 +663,7 @@ lemma sound_optimize_noop:
   "eval_match m s = eval_match (elim_noop m) s"
   apply (induction m arbitrary: s rule: elim_noop.induct)
   using noop_semantics_rhs apply force+
-  using seq_det_rhs apply force+
-  using elim_noop.simps(23) elim_noop.simps(46) seq_det_rhs apply presburger
-  by force+
+  using seq_det_rhs by force+
 
 (*lemma monotonic_choice:
   assumes "\<forall> r e. eval_rules r u e = eval_rules (f r) u e"
@@ -704,12 +730,12 @@ lemma eliminate_noop_valid:
   by (smt (verit) Rules.distinct(11) Rules.distinct(15) Rules.distinct(19) Rules.distinct(5) Rules.inject(4) eliminate_noop.simps(5) eval_rules.simps)
 
 fun elim_empty :: "MATCH \<Rightarrow> MATCH" where
-  "elim_empty (check Empty) = noop" |
+  "elim_empty (condition Empty) = noop" |
   "elim_empty (m1 && m2) = (elim_empty m1 && elim_empty m2)" |
   "elim_empty m = m"
 
 lemma empty_check_semantics:
-  "eval_match (check Empty) s = eval_match noop s"
+  "eval_match (condition Empty) s = eval_match noop s"
   by simp
 
 lemma sound_optimize_empty:
@@ -749,7 +775,7 @@ fun combined_size :: "Rules \<Rightarrow> nat" where
   "combined_size (choice []) = 1" |
   "combined_size (r1 \<then> r2) = combined_size r1 + combined_size r2"
 
-value "size noop"
+value "size (m ? r)"
 
 function (sequential) lift_match :: "Rules \<Rightarrow> Rules" where
   "lift_match (r1 else r2) = ((lift_match r1) else (lift_match r2))" |
@@ -790,10 +816,8 @@ lemma lift_match_valid:
   apply (metis (full_types) condE eval_rules.intros(2) eval_rules.intros(3) lift_match.simps(5))
       apply (metis (full_types) condE eval_rules.intros(2) eval_rules.intros(3) lift_match.simps(6))
      apply (metis (full_types) condE eval_rules.intros(2) eval_rules.intros(3) lift_match.simps(7))
-    apply (metis (full_types) condE eval_rules.intros(2) eval_rules.intros(3) lift_match.simps(8))
-   apply (metis (full_types) condE eval_rules.intros(2) eval_rules.intros(3) lift_match.simps(9))
-   apply simp
-  by (smt (verit) Rules.distinct(11) Rules.distinct(15) Rules.distinct(19) Rules.distinct(5) Rules.inject(4) eval_rules.simps lift_match.simps(11))
+   apply simp+
+  by (smt (verit) Rules.distinct(11) Rules.distinct(15) Rules.distinct(19) Rules.distinct(5) Rules.inject(4) eval_rules.simps)
 
 (*
 fun lift_common :: "Rules \<Rightarrow> Rules" where
@@ -858,28 +882,438 @@ termination
   apply auto[1] using join_conditions_shrinks apply (simp add: le_imp_less_Suc size_list_estimation')
   by simp+
 
-lemma match_eq:
-  "eval_match (m && m) u = eval_match m u"
-  sorry
+fun pattern_variables :: "PatternExpr \<Rightarrow> String.literal set" where
+  "pattern_variables (UnaryPattern op e) = {e}" |
+  "pattern_variables (BinaryPattern op e1 e2) = {e1, e2}" |
+  "pattern_variables (ConditionalPattern c t f) = {c, t, f}" |
+  "pattern_variables (VariablePattern v) = {v}" |
+  "pattern_variables (ConstantPattern v) = {}" |
+  "pattern_variables (ConstantVarPattern v) = {v}"
 
+fun match_variables :: "MATCH \<Rightarrow> String.literal set" where
+  "match_variables (match v p) = {v} \<union> pattern_variables p" |
+  "match_variables (equality e1 e2) = {e1, e2}" |
+  "match_variables (m1 && m2) = match_variables m1 \<union> match_variables m2" |
+  "match_variables (condition c) = {}" |
+  "match_variables noop = {}"
+
+fun valid_match :: "MATCH \<Rightarrow> bool" where
+  "valid_match (match v (UnaryPattern op e)) = (v \<noteq> e)" |
+  "valid_match (match v (BinaryPattern op e1 e2)) = (v \<noteq> e1 \<and> v \<noteq> e2 \<and> e1 \<noteq> e2)" |
+  "valid_match (match v (ConditionalPattern c t f)) = (v \<noteq> c \<and> v \<noteq> t \<and> v \<noteq> f \<and> c \<noteq> t \<and> c \<noteq> f \<and> t \<noteq> f)" |
+  "valid_match (m1 && m2) = (valid_match m1 \<and> valid_match m2 \<and> match_variables m1 \<inter> match_variables m2 = {})" |
+  "valid_match _ = True"
+
+fun valid_rules :: "Rules \<Rightarrow> bool" where
+  "valid_rules (m ? r) = (valid_match m \<and> valid_rules r)" |
+  "valid_rules (r1 else r2) = (valid_rules r1 \<and> valid_rules r2)" |
+  "valid_rules (r1 \<then> r2) = (valid_rules r1 \<and> valid_rules r2)" |
+  "valid_rules (choice rules) = (\<forall>r \<in> set rules. valid_rules r)" |
+  "valid_rules _ = True"
+
+experiment begin
+lemma match_affect:
+  assumes "eval_match m u = Some a"
+  shows "\<forall>v. v \<notin> match_variables m \<longrightarrow> u v = a v"
+using assms proof (induction m u arbitrary: a rule: eval_match.induct)
+  case (1 v op1 x s)
+  have "match_variables (MATCH.match v (UnaryPattern op1 x)) = {v, x}"
+    by auto
+  have "\<exists>e. a = s(x\<mapsto>e)"
+    by (smt (verit, ccfv_threshold) "1" IRExpr.case_eq_if eval_match.simps(1) option.case_eq_if option.distinct(1) option.inject)
+  then show ?case
+    by fastforce
+next
+  case (2 v op1 x y s)
+  then show ?case sorry
+next
+  case (3 v c tb fb s)
+  then show ?case sorry
+next
+  case (4 v c1 s)
+  then show ?case sorry
+next
+  case (5 v1 v2 s)
+  then show ?case sorry
+next
+  case (6 m1 m2 s)
+  then show ?case sorry
+next
+  case (7 s)
+  then show ?case sorry
+next
+  case (8 sc s)
+  then show ?case sorry
+next
+  case ("9_1" v vb s)
+  then show ?case sorry
+next
+  case ("9_2" v vb s)
+  then show ?case sorry
+qed
+
+lemma idempotent_match:
+  assumes "valid_match m"
+  assumes "eval_match m u = Some a"
+  shows "eval_match m a = Some a"
+  using assms proof (induction m u arbitrary: u a rule: eval_match.induct)
+  case (1 v op1 x s)
+  then obtain e where e: "u v = Some (UnaryExpr op1 e)"
+    by (smt (verit) IRExpr.case_eq_if IRExpr.sel(1) eval_match.simps(1) is_UnaryExpr_def map_upd_Some_unfold option.case_eq_if option.distinct(1) option.exhaust_sel option.sel valid_match.simps(1))
+    then have "a = u(x:=Some e)"
+        using "1.prems"(2) by auto
+    then show ?case
+      using "1.prems"(1) e by auto
+next
+  case (2 v op1 x y s)
+  then show ?case sorry
+  (*then obtain e1 e2 where e: "u v = Some (BinaryExpr op1 e1 e2)"
+    by (smt (verit, del_insts) IRExpr.case_eq_if IRExpr.simps(66) eval_match.simps(2) is_BinaryExpr_def option.case_eq_if option.distinct(1) option.exhaust_sel)
+  then have "s = u(x:=Some e1, y:=Some e2)"
+    using "2.prems"(2) by auto
+  then show ?case
+    using "2.prems"(1) e by auto*)
+next
+  case (3 v c tb fb s)
+  then show ?case sorry
+  (*then obtain cv t f where e: "u v = Some (ConditionalExpr cv t f)"
+    unfolding eval_match.simps
+    by (smt (verit, del_insts) IRExpr.split_sel_asm is_none_code(2) is_none_simps(1) option.case_eq_if option.exhaust_sel)
+  then have "s = u(c:=Some cv, tb:=Some t, fb:=Some f)"
+    using "3.prems"(2) by auto
+  then show ?case
+    using "3.prems"(1) e by auto*)
+next
+  case (4 v c1 s)
+  then show ?case unfolding eval_match.simps
+    by (smt (verit) IRExpr.case_eq_if option.case_eq_if option.sel)
+next
+  case (5 v1 v2 s)
+  then show ?case unfolding eval_match.simps
+    by (metis option.inject)
+next
+  case (6 m1 m2 s)
+  (*obtain a' u where a': "eval_match m1 u = Some a'"
+    using "6.prems"(2) by fastforce
+  then have s1: "eval_match m1 u = Some a'"
+    using "6.IH"(1) "6.prems"(1) valid_match.simps(4) by blast
+  obtain a'' where a'': "eval_match m2 u = Some a''"
+    using "6.prems"(2) \<open>eval_match m1 u = Some a'\<close> by auto
+  then have s2: "eval_match m2 a'' = Some a''"
+    using "6.IH"(2) "6.prems"(1) \<open>eval_match m1 s = Some a'\<close> valid_match.simps(4) by blast
+  have "a = a''"
+    using "6.prems"(2) a' a'' by auto
+  have "eval_match m1 a = Some a"
+    sorry*)
+  then show ?case sorry(*using "6.prems"(2) unfolding eval_match.simps
+    by (simp add: \<open>a = a''\<close> s2)*)
+next
+  case (7 s)
+  then show ?case sorry
+next
+  case (8 sc s)
+  then show ?case sorry
+next
+  case ("9_1" v vb s)
+  then show ?case sorry
+next
+  case ("9_2" v vb s)
+  then show ?case sorry
+qed
+
+lemma match_eq:
+  assumes "valid_match m"
+  shows "eval_match (m && m) u = eval_match m u"
+proof (cases "eval_match m u")
+  case None
+  then show ?thesis by simp
+next
+  case (Some a)
+  then have "eval_match m a = eval_match m u"
+    using assms proof (induction m a arbitrary: a rule: eval_match.induct)
+    case (1 v op1 x s)
+      then show ?case
+      proof (cases "\<exists>e. u v = Some (UnaryExpr op1 e)")
+        case True
+        obtain e where "a x = Some e"
+          using "1" True by fastforce
+        then have "x \<noteq> v"
+          using assms
+          using "1.prems"(2) by force
+        then have "a = u(x:=Some e)"
+          using "1.prems"(1) True \<open>a x = Some e\<close> by force
+        then show ?thesis unfolding eval_match.simps
+          using True \<open>x \<noteq> v\<close> by force
+      next
+        case False
+        then have "eval_match (MATCH.match v (UnaryPattern op1 x)) u = None"
+          unfolding eval_match.simps
+          by (smt (verit, best) IRExpr.case_eq_if IRExpr.sel(1) is_UnaryExpr_def option.case_eq_if option.exhaust_sel)
+        then show ?thesis
+          using "1.prems"(1) by auto
+      qed
+    next
+      case (2 v op1 x y s)
+      then show ?case
+      proof (cases "\<exists>e1 e2. u v = Some (BinaryExpr op1 e1 e2)")
+        case True
+        then obtain e1 e2 where e: "u v = Some (BinaryExpr op1 e1 e2)"
+          by blast
+        then have e2: "a y = Some e2"
+          using "2"(1) unfolding eval_match.simps
+          by auto
+        have e1: "a x = Some e1"
+          using "2.prems"(1) "2.prems"(2) e by auto
+        then have "x \<noteq> v \<and> y \<noteq> v"
+          using assms
+          using "2.prems"(2) by auto
+        then have "a = (u(y:=Some e2))(x:=Some e1)"
+          using e1 e2 "2"(1) unfolding eval_match.simps using True
+          by (smt (verit, ccfv_threshold) IRExpr.simps(66) e fun_upd_idem fun_upd_other fun_upd_twist map_add_subsumed1 map_add_upd map_le_refl option.inject option.simps(5))
+        then show ?thesis unfolding eval_match.simps
+          by (smt (z3) "2.prems"(1) IRExpr.simps(66) \<open>x \<noteq> v \<and> y \<noteq> v\<close> e e2 eval_match.simps(2) fun_upd_apply fun_upd_triv map_add_subsumed2 map_le_refl option.case_eq_if option.sel)
+      next
+        case False
+        then have "eval_match (MATCH.match v (BinaryPattern op1 x y)) u = None"
+          unfolding eval_match.simps
+          using IRExpr.case_eq_if IRExpr.sel(2) is_BinaryExpr_def option.case_eq_if option.exhaust_sel
+          by (smt (verit) IRExpr.simps(66))
+        then show ?thesis
+          using "2.prems"(1) by force
+      qed
+    next
+      case (3 v c tb fb s)
+      then show ?case
+      proof (cases "\<exists>cv t f. u v = Some (ConditionalExpr cv t f)")
+        case True
+        then obtain cv t f where e: "u v = Some (ConditionalExpr cv t f)"
+          by blast
+        then have f: "a fb = Some f"
+          using "3.prems"(1) unfolding eval_match.simps
+          by force
+        then have t: "a tb = Some t"
+          using "3.prems"(1,2) unfolding eval_match.simps
+          using e by auto
+        then have c: "a c = Some cv"
+          using "3.prems"(1,2) unfolding eval_match.simps
+          using e by auto
+        then have "c \<noteq> v \<and> tb \<noteq> v \<and> tb \<noteq> v"
+          using assms
+          using "3.prems"(2) by auto
+        then have "a = ((u(c:=Some cv))(tb:=Some t))(fb:=Some f)"
+          using c t f "3"(1) unfolding eval_match.simps using True
+          using e by auto
+        then show ?thesis unfolding eval_match.simps
+          using "3.prems"(2) e by auto
+      next
+        case False
+        then have "eval_match (MATCH.match v (ConditionalPattern c tb fb)) u = None"
+          unfolding eval_match.simps
+          using IRExpr.split_sels(2) is_none_code(2) is_none_simps(1) option.case_eq_if option.exhaust_sel
+          by (smt (verit, del_insts))
+        then show ?thesis
+          using "3.prems"(1) by force
+      qed
+    next
+      case (4 v c1 s)
+      then show ?case unfolding eval_match.simps
+        using IRExpr.case_eq_if option.case_eq_if option.sel
+        by (smt (verit))
+    next
+      case (5 v1 v2 s)
+      then show ?case
+        by (metis eval_match.simps(5) option.sel)
+    next
+      case (6 m1 m2 s)
+      then show ?case
+      proof (cases "eval_match m1 u")
+        case None
+        then show ?thesis
+          using "6.prems"(1) by force
+      next
+        case (Some a')
+        then show ?thesis sorry
+      qed
+        (*
+      proof (cases "eval_match (m1 && m2) u")
+        case None
+        then show ?thesis
+          using "6.prems"(1) by auto
+      next
+        case (Some a)
+        have "eval_match m1 u = Some s" sorry
+        then show ?thesis sorry
+      qed*)
+    next
+      case (7 s)
+      then show ?case sorry
+    next
+      case (8 sc s)
+      then show ?case sorry
+    next
+      case ("9_1" v vb s)
+      then show ?case sorry
+    next
+      case ("9_2" v vb s)
+      then show ?case sorry
+    qed
+  then show ?thesis
+    by (simp add: Some)
+qed
+end
+(*
+      case (match x1 x2)
+      then show ?case sorry
+    next
+      case (equality x1 x2)
+      then have "a = u"
+        using Some unfolding eval_match.simps
+        by (metis option.distinct(1) option.inject)
+      then show ?case by simp
+    next
+      case (andthen m1 m2)
+      then show ?case 
+      proof (cases "eval_match m1 u = None")
+        case True
+        then show ?thesis
+          using andthen.prems by auto
+      next
+        case False
+        then obtain u' where "eval_match m1 u = Some u'"
+          by force
+        then have "eval_match m2 u' = Some a"
+          using andthen unfolding eval_match.simps
+          by simp
+        then show ?thesis sorry
+      qed
+        unfolding eval_match.simps
+    next
+      case (condition x)
+      then have "a = u"
+        using Some unfolding eval_match.simps
+        by (metis option.distinct(1) option.inject)
+      then show ?case by simp
+    next
+      case noop
+      then show ?case by simp
+    qed
+  then show ?thesis
+    by (simp add: Some)
+qed
+*)
+
+lemma monotonic_cond:
+  assumes "\<forall>e u. eval_rules r u e = eval_rules (f r) u e"
+  shows "\<forall>e u. eval_rules (m ? r) u e = eval_rules (m ? f r) u e"
+  using assms by (metis condE eval_rules.intros(2) eval_rules.intros(3))
+
+lemma monotonic_else:
+  assumes "\<forall>e u. eval_rules r1 u e = eval_rules (f r1) u e"
+  assumes "\<forall>e u. eval_rules r2 u e = eval_rules (f r2) u e"
+  shows "\<forall>e. eval_rules (r1 else r2) u e = eval_rules (f r1 else f r2) u e"
+  using assms
+  by (metis elseE eval_rules.intros(4) eval_rules.intros(5))
+
+lemma monotonic_seq:
+  assumes "\<forall>e u. eval_rules r1 u e = eval_rules (f r1) u e"
+  assumes "\<forall>e u. eval_rules r2 u e = eval_rules (f r2) u e"
+  shows "\<forall>e. eval_rules (r1 \<then> r2) u e = eval_rules (f r1 \<then> f r2) u e"
+  using assms
+  by (smt (verit) eval_rules.simps seqE)
+
+lemma monotonic_choice:
+  assumes "\<forall>r e u. r \<in> set rules \<longrightarrow> eval_rules r u e = eval_rules (f r) u e"
+  shows "\<forall>e. eval_rules (choice rules) u e = eval_rules (choice (map f rules)) u e"
+  using assms apply (induction rules) apply simp
+  by (metis choice_join list.set_intros(1) list.set_intros(2))
+
+experiment begin
 lemma redundant_conditions:
-  "eval_rules (m ? (m ? r1)) u e = eval_rules (m ? r1) u e"
-  using match_eq chain_equiv
-  by (smt (verit, best) condE eval_rules.intros(2) eval_rules.intros(3))
+  assumes "valid_match m"
+  shows "eval_rules (m ? (m ? r1)) u e = eval_rules (m ? r1) u e" (is "?lhs = ?rhs")
+proof -
+  have "?lhs = eval_rules ((m && m) ? r1) u e"
+    using chain_equiv
+    by simp
+  moreover have "eval_rules ((m && m) ? r1) u e = ?rhs"
+    sorry
+    (*using match_eq
+    by (smt (verit) Rules.distinct(1) Rules.distinct(11) Rules.distinct(13) Rules.distinct(9) Rules.inject(2) assms eval_rules.simps)
+    *)
+  ultimately show ?thesis by simp
+qed
 
 lemma join_conditions_valid:
-  "join_conditions r = Some r' \<Longrightarrow> eval_rules r u e = eval_rules r' u e"
-  apply (induction r rule: join_conditions.induct)
+  assumes "valid_rules r"
+  shows "join_conditions r = Some r' \<Longrightarrow> eval_rules r u e = eval_rules r' u e"
+  using assms apply (induction r rule: join_conditions.induct)
   apply (smt (verit, ccfv_threshold) condE elseE eval_rules.intros(2) eval_rules.intros(3) eval_rules.intros(4) eval_rules.intros(5) join_conditions.simps(1) option.distinct(1) option.sel)
-  apply (metis join_conditions.simps(2) option.discI option.inject redundant_conditions)
+  subgoal premises p for m1 m2 r
+  proof -
+    have v1:"valid_match m1" using p(2) by simp
+    moreover have v2:"valid_match m2" using p(2) by simp
+    ultimately show ?thesis
+      by (metis join_conditions.simps(2) option.discI option.sel p(1) redundant_conditions)
+  qed
   by simp+
 
 lemma lift_common_valid:
-  "eval_rules r u e = eval_rules (lift_common r) u e"
-  apply (induction r arbitrary: u e rule: lift_common.induct)
-    subgoal for r1 r2 apply (cases "join_conditions (r1 else r2)")
-    apply (smt (verit, del_insts) elseE eval_rules.intros(4) eval_rules.intros(5) lift_common.simps(1) option.simps(4))
-      by (simp add: join_conditions_valid)
+  assumes "valid_rules r"
+  shows "eval_rules r u e = eval_rules (lift_common r) u e"
+  using assms proof (induction r arbitrary: u e rule: lift_common.induct)
+  case (1 r1 r2)
+  then show ?case
+  proof (cases "join_conditions (r1 else r2)")
+    case None
+    then have "(lift_common (r1 else r2)) = (lift_common r1 else lift_common r2)"
+      by simp
+    then show ?thesis using 1
+      by (simp add: None monotonic_else)
+  next
+    case (Some a)
+    then obtain m1 m2 r1' r2' where ex: "(r1 else r2) = (m1 ? r1' else m2 ? r2')"
+      by (metis eliminate_empty.cases join_conditions.simps(10) join_conditions.simps(11) join_conditions.simps(12) join_conditions.simps(13) join_conditions.simps(14) join_conditions.simps(15) join_conditions.simps(8) join_conditions.simps(9) option.distinct(1))
+    then have "m1 = m2"
+      by (metis Some join_conditions.simps(1) option.distinct(1))
+    then show ?thesis using 1
+      using ex join_conditions_valid by auto
+  qed
+next
+  case (2 m r)
+  then show ?case
+  proof (cases "join_conditions (m ? r)")
+    case None
+    then have "(lift_common (m ? r)) = (m ? lift_common r)"
+      by simp
+    then show ?thesis using 2
+      by (simp add: None monotonic_cond)
+  next
+    case (Some a)
+    then obtain m1 m2 r' where ex: "(m ? r) = (m1 ? (m2 ? r'))"
+      by (smt (z3) Rules.distinct(9) join_conditions.elims option.distinct(1))
+    then have "m1 = m2"
+      by (metis Some join_conditions.simps(2) option.distinct(1))
+    then show ?thesis using 2
+      by (simp add: ex join_conditions_valid)
+  qed
+next
+  case (3 rules)
+  then show ?case by (simp add: monotonic_choice)
+next
+  case (4 e)
+  then show ?case by simp
+next
+  case (5 r1 r2)
+  then show ?case by (simp add: monotonic_seq)
+qed
+end
+  (*subgoal for r1 r2 apply (cases "join_conditions (r1 else r2)")
+    apply (smt (verit, del_insts) elseE eval_rules.intros(4) eval_rules.intros(5) lift_common.simps(1) option.case_eq_if valid_rules.simps(2))
+    unfolding lift_common.simps valid_rules.simps 
+    using join_conditions_valid sledgehammer
+    using join_conditions.elims join_conditions_valid lift_common.simps(1) option.distinct(1) option.simps(5) valid_rules.simps(1) valid_rules.simps(2)
+    *)
+(*
     subgoal for m r u apply (cases "join_conditions (m ? r)")
        apply simp apply (metis condE eval_rules.intros(2) eval_rules.intros(3))
       by (simp add: join_conditions_valid)
@@ -888,6 +1322,15 @@ lemma lift_common_valid:
       by (metis choice_join lift_common.simps(3) list.set_intros(1) list.set_intros(2))
      apply simp
     by (smt (verit) Rules.distinct(11) Rules.distinct(15) Rules.distinct(19) Rules.distinct(5) Rules.inject(4) eval_rules.simps lift_common.simps(5))
+*)
+
+fun common_size :: "Rules \<Rightarrow> nat" where
+  "common_size (m ? r) = 1 + common_size r" |
+  "common_size (base e) = 0" |
+  "common_size (r1 else r2) = 1 + common_size r1 + common_size r2" |
+  "common_size (choice (rule # rules)) = 1 + common_size rule + common_size (choice rules)" |
+  "common_size (choice []) = 0" |
+  "common_size (r1 \<then> r2) = 1 + common_size r1 + common_size r2"
 
 fun find_common :: "MATCH \<Rightarrow> Rules \<Rightarrow> Rules option" where
   "find_common m (m' ? r) = (if m = m' then Some r else None)" |
@@ -900,25 +1343,156 @@ fun find_uncommon :: "MATCH \<Rightarrow> Rules \<Rightarrow> Rules option" wher
 definition join_common :: "MATCH \<Rightarrow> Rules list \<Rightarrow> Rules list" where
   "join_common m rules = List.map_filter (find_common m) rules"
 
+lemma find_common_defn:
+  assumes "find_common m x = v"
+  shows "v \<noteq> None \<longleftrightarrow> (\<exists>r. x = (m ? r) \<and> v = Some r)"
+  using assms apply (induction m x rule: find_common.induct) unfolding find_common.simps apply force
+  by simp+
+
+lemma find_common_shrinks:
+  "find_common m x = Some z \<Longrightarrow> common_size z \<le> common_size x"
+  unfolding find_common.simps using find_common_defn
+  by (metis common_size.simps(1) le_add2 option.distinct(1) option.inject)
+
+lemma join_common_shrinks:
+  "common_size (choice (join_common m x)) \<le> common_size (choice x)"
+  unfolding join_common_def
+  apply (induction x)
+   apply (simp add: map_filter_simps(2))
+  subgoal for a x
+    apply (cases "find_common m a") unfolding List.map_filter_def apply simp
+    using find_common_shrinks apply simp
+    using add_le_mono by blast
+  done
+
 definition join_uncommon :: "MATCH \<Rightarrow> Rules list \<Rightarrow> Rules list" where
   "join_uncommon m rules = List.map_filter (find_uncommon m) rules"
 
+lemma find_uncommon_preserve:
+  "find_uncommon m r = Some r \<or> find_uncommon m r = None"
+  by (metis find_uncommon.elims)
+
+lemma join_uncommon_subset:
+  "set (join_uncommon m x) \<subseteq> set x"
+  unfolding join_uncommon_def List.map_filter_def using find_uncommon_preserve
+  by (smt (verit, best) comp_def filter_is_subset list.map_ident_strong mem_Collect_eq option.sel set_filter)
+
 lemma size_join_uncommon:
-  "size (join_uncommon m rules) \<le> size rules"
+  "\<forall>r \<in> set (join_uncommon m rules) . find_uncommon m r = Some r' \<longrightarrow> common_size r' \<le> common_size r"
   unfolding join_uncommon_def map_filter_def
-  by (induction rule: find_uncommon.induct; auto)
+  apply (induction rule: find_uncommon.induct; auto)
+     apply (metis common_size.simps(1) find_uncommon_preserve le_Suc_eq option.inject plus_1_eq_Suc)
+    apply (metis Suc_eq_plus1_left add.assoc common_size.simps(3) find_uncommon_preserve option.inject verit_comp_simplify1(2))
+   apply (metis Suc_eq_plus1_left add.assoc common_size.simps(6) find_uncommon_preserve option.inject order_refl)
+  by (metis find_uncommon_preserve option.inject order_refl)
+
+lemma find_uncommon_shrinks:
+  "find_uncommon m x = Some z \<Longrightarrow> common_size z \<le> common_size x"
+  unfolding find_uncommon.simps
+  by (metis dual_order.refl find_uncommon_preserve option.distinct(1) option.inject)
+
+lemma join_uncommon_shrinks:
+  "common_size (choice (join_uncommon m rules))
+       \<le> (common_size (choice rules))"
+  unfolding join_uncommon_def
+  apply (induction rules)
+   apply (simp add: map_filter_simps(2))
+  subgoal for a x
+    apply (cases "find_uncommon m a") unfolding List.map_filter_def apply simp
+    using find_uncommon_shrinks
+    by (simp add: add_le_mono dual_order.refl)
+  done
 
 function (sequential) combine_conditions :: "Rules \<Rightarrow> Rules" where
   "combine_conditions (base e) = base e" |
   "combine_conditions (r1 else r2) = (combine_conditions r1 else combine_conditions r2)" |
   "combine_conditions (m ? r) = (m ? combine_conditions r)" |
   "combine_conditions (choice ((m ? r) # rules)) = 
-    choice ((m ? combine_conditions (choice (r # join_common m rules))) # map combine_conditions (join_uncommon m rules))" |
+    choice ((m ? combine_conditions (choice (r # join_common m rules)))
+      # [combine_conditions (choice (join_uncommon m rules))])" |
   "combine_conditions (choice rules) = 
     choice (map combine_conditions rules)" |
   "combine_conditions (r1 \<then> r2) = (combine_conditions r1 \<then> combine_conditions r2)"
   apply pat_completeness+
   by simp+
+
+experiment begin
+\<comment> \<open>Can we define a version of the optimization over a list?\<close>
+\<comment> \<open>Not like this, still requires recursing on the subparts in combine\_conditions\_list\<close>
+fun combine_conditions_list :: "Rules list \<Rightarrow> Rules list" where
+  "combine_conditions_list ((m ? r) # rules) =
+    ((m ? (choice (r # join_common m rules))) # (join_uncommon m rules))" |
+  "combine_conditions_list r = r"
+
+lemma "x \<in> set (combine_conditions_list rules) \<Longrightarrow> common_size x < common_size (choice rules)"
+  apply (induction rules rule: combine_conditions_list.induct) 
+  unfolding combine_conditions_list.simps
+  unfolding join_common_def join_uncommon_def List.map_filter_def
+  apply simp sorry
+
+function (sequential) combine_conditions2 :: "Rules \<Rightarrow> Rules" where
+  "combine_conditions2 (base e) = base e" |
+  "combine_conditions2 (r1 else r2) = (combine_conditions2 r1 else combine_conditions2 r2)" |
+  "combine_conditions2 (m ? r) = (m ? combine_conditions2 r)" |
+  "combine_conditions2 (choice rules) =
+    choice (map combine_conditions2 (combine_conditions_list rules))" |
+  "combine_conditions2 (r1 \<then> r2) = (combine_conditions2 r1 \<then> combine_conditions2 r2)"
+  apply pat_completeness+
+  by simp+
+
+termination combine_conditions2
+  apply (relation "measures [common_size, size]") apply auto[1] apply simp+ using join_common_shrinks
+  sorry
+end
+
+experiment begin
+\<comment> \<open>Can we define combine conditions in a two step process: 1) group matches 2) pull out matching m's\<close>
+
+fun find_common_unchanged :: "MATCH \<Rightarrow> Rules \<Rightarrow> Rules option" where
+  "find_common_unchanged m (m' ? r) = (if m = m' then Some (m' ? r) else None)" |
+  "find_common_unchanged m r = None"
+
+definition group_common :: "MATCH \<Rightarrow> Rules list \<Rightarrow> Rules list" where
+  "group_common m rules = List.map_filter (find_common_unchanged m) rules"
+
+function (sequential) group_conditions :: "Rules \<Rightarrow> Rules" where
+  "group_conditions (base e) = base e" |
+  "group_conditions (r1 else r2) = (group_conditions r1 else group_conditions r2)" |
+  "group_conditions (m ? r) = (m ? group_conditions r)" |
+  "group_conditions (choice ((m ? r) # rules)) = 
+    choice ((group_conditions (choice ((m ? r) # group_common m rules)))
+      # [group_conditions (choice (join_uncommon m rules))])" |
+  "group_conditions (choice rules) = 
+    choice (map group_conditions rules)" |
+  "group_conditions (r1 \<then> r2) = (group_conditions r1 \<then> group_conditions r2)"
+  apply pat_completeness+
+  by simp+
+
+termination group_conditions
+  apply (relation "measures [common_size, size]") apply auto[1] apply simp+ using join_common_shrinks
+  sorry
+
+function (sequential) merge_conditions :: "Rules \<Rightarrow> Rules" where
+  "merge_conditions (base e) = base e" |
+  "merge_conditions (r1 else r2) = (merge_conditions r1 else merge_conditions r2)" |
+  "merge_conditions (m ? r) = (m ? merge_conditions r)" |
+  "merge_conditions (choice ((m ? r) # (m' ? r') # rules)) = (if m = m' then
+    m ? choice (map merge_conditions (r # r' # join_common m rules)) else
+    choice (map merge_conditions ((m ? r) # (m' ? r') # rules)))" |
+  "merge_conditions (choice rules) = 
+    choice (map merge_conditions rules)" |
+  "merge_conditions (r1 \<then> r2) = (merge_conditions r1 \<then> merge_conditions r2)"
+  apply pat_completeness+
+  by simp+
+
+termination merge_conditions
+  apply (relation "measures [common_size, size]") apply auto[1] apply simp+ using join_common_shrinks
+  sorry
+
+definition collapse_conditions :: "Rules \<Rightarrow> Rules" where
+  "collapse_conditions = merge_conditions o group_conditions"
+
+end
 
 lemma find_common_size:
   assumes "(find_common m r) \<noteq> None"
@@ -932,7 +1506,7 @@ lemma "size_list size (join_common m rules) \<le> (size_list size rules)"
   (*apply (induction rules) apply auto[1]*)
   apply (induction rule: find_common.induct)
   apply (induction rules) 
-  apply simp using find_common_size sledgehammer
+  apply simp using find_common_size sorry
 
 lemma
   "combined_size (choice (join_common m rules))
@@ -940,34 +1514,822 @@ lemma
        combined_size (choice (join_common m rules)) =
        combined_size (m ? (choice rules)) \<and>
        size_list size (join_common m rules) < Suc (size_list size rules)"
+*)
+
+lemma common_size_choice_gt:
+  "x \<in> set va \<Longrightarrow> common_size x \<le> common_size (choice va)"
+  apply (induction va) apply simp
+  by fastforce
 
 termination combine_conditions
-  apply (relation "measures [combined_size, size]") apply auto[1] apply simp+
-  apply blast+
-  apply fastforce+ apply simp unfolding join_common_def sledgehammer
+  apply (relation "measures [common_size]") apply auto[1] apply simp+ using join_common_shrinks
+          apply (simp add: le_imp_less_Suc) defer
+         apply simp apply auto[1]
+        apply (simp add: common_size_choice_gt le_imp_less_Suc)
+       apply auto[1] using common_size_choice_gt apply fastforce
+      apply auto[1] using common_size_choice_gt apply fastforce
+     apply auto[1] using common_size_choice_gt apply fastforce
+    apply simp+ using join_uncommon_shrinks
+  by (metis le_imp_less_Suc plus_1_eq_Suc trans_le_add2)
+
+lemma join_common_empty: "join_common m [] = []"
+  by (simp add: join_common_def map_filter_simps(2))
+lemma join_uncommon_empty: "join_uncommon m [] = []"
+  by (simp add: join_uncommon_def map_filter_simps(2))
+
+(*
+lemma eval_choice: "eval_rules (choice rules) u e \<longrightarrow> (\<exists> r \<in> set rules . eval_rules r u e)"
+  sorry
+*)
+
+lemma eval_choice: "{e. eval_rules (choice rules) u e \<and> e \<noteq> None} = {e | e r . r \<in> set rules \<and> eval_rules r u e \<and> e \<noteq> None}"
+  using choiceE eval_rules.intros(6) by fastforce
+
+lemma eval_choice_none: "eval_rules (choice rules) u None = (\<forall> r \<in> set rules . eval_rules r u None)"
+  by (metis choiceE eval_rules.intros(7) length_pos_if_in_set list.size(3) nless_le option.distinct(1))
+
+inductive_cases evalRulesE: "eval_rules r u e"
+
+lemma eval_always_result:
+  "\<exists> e. eval_rules r u e"
+  apply (induction r arbitrary: u)
+  using eval_rules.intros(1) apply auto[1]
+  using eval_rules.intros(2,3) apply (meson opt_to_list.cases) 
+  using eval_rules.intros(4,5) apply (metis split_option_ex) 
+  using eval_rules.intros(9,10) apply (metis split_option_ex) 
+  using eval_rules.intros(6,7,8) by (metis split_option_ex) 
+
+experiment begin
+lemma eval_choice_none_always:
+  assumes "eval_rules (choice rules) u None"
+  assumes "rules \<noteq> []"
+  shows "(\<forall>r. eval_rules (choice rules) u r \<longrightarrow> r = None)"
+  sorry
+  (*using assms apply (subst (asm) eval_choice_none)
+  apply (rule allI)
+  subgoal for r
+    using assms evalRulesE
+  apply (induction rule: eval_rules.induct)
+  using baseE apply blast
+  apply (metis condE option.distinct(1) option.sel) 
+  apply (metis condE option.distinct(1))
+  apply (metis elseE option.distinct(1))
+  apply (metis elseE option.distinct(1)) using eval_choice_none *)
+
+lemma eval_choice_some_e:
+  assumes "eval_rules (choice rules) u e"
+  assumes "e \<noteq> None"
+  shows "(\<exists>r \<in> set rules. eval_rules r u e)"
+  by (metis assms(1) assms(2) choiceE)
+
+lemma eval_single_choice: "{e. eval_rules (choice [r]) u e} = {e. eval_rules r u e}" (is "?lhs = ?rhs")
+proof (cases "eval_rules r u None")
+  case True
+  then have "eval_rules (choice [r]) u None"
+    by (simp add: eval_rules.intros(7))
+  then show ?thesis
+    by (metis True eval_choice_none_always eval_rules.intros(6) list.distinct(1) list.set_intros(1) option.exhaust)
+next
+  case False
+  then have "\<forall>e. eval_rules r u (Some e) \<longrightarrow> eval_rules (choice [r]) u (Some e)"
+    by (simp add: eval_rules.intros(6))
+  also have "\<forall>e. eval_rules (choice [r]) u (Some e) \<longrightarrow> eval_rules r u (Some e)"
+    using eval_choice_some_e by force
+  then show ?thesis
+    by (metis False calculation eval_always_result eval_choice_none_always not_Cons_self2 not_None_eq)
+qed
+
+lemma monotonic_choice:
+  assumes "\<forall>r \<in> set rules. {e. eval_rules r u e} = {e. eval_rules (f r) u e}"
+  shows "{e. eval_rules (choice rules) u e} = {e. eval_rules (choice (map f rules)) u e}"
+proof (cases "eval_rules (choice rules) u None")
+  case True
+  then have "\<forall>r \<in> set rules. eval_rules r u None"
+    by (simp add: eval_choice_none)
+  then have "\<forall>r \<in> set rules. eval_rules (f r) u None"
+    using assms by blast
+  then have "eval_rules (choice (map f rules)) u None"
+    using eval_choice_none sorry
+  then show ?thesis
+    by (metis Nil_is_map_conv True eval_choice_none_always)
+next
+  case False
+  then have "\<forall>e. eval_rules (choice rules) u (Some e) \<longrightarrow> eval_rules (choice (map f rules)) u (Some e)"
+    sorry
+  also have "\<forall>e. eval_rules (choice (map f rules)) u (Some e) \<longrightarrow> eval_rules (choice rules) u (Some e)"
+    sorry
+  then show ?thesis
+    by (metis Nil_is_map_conv calculation choiceE eval_always_result eval_choice_none_always)
+qed
+  
+
+lemma combine_no_recurse:
+  "{e. eval_rules (choice ((m ? r) # rules)) u e} = {e. eval_rules 
+  (choice [(m ? (choice (r # join_common m rules))), choice (join_uncommon m rules)]) u e}"
+  (is "{e. eval_rules ?lhs u e} = {e. eval_rules ?rhs u e}")
+proof (induction rules)
+  case Nil
+  have "(choice ((m ? choice (r # join_common m [])) # join_uncommon m [])) = choice ([m ? choice [r]])"
+    using join_common_empty join_uncommon_empty
+    by simp
+  also have "{e. eval_rules (choice ([m ? choice [r]])) u e} = {e. eval_rules (m ? r) u e}"
+    using eval_single_choice
+    by (smt (z3) Collect_cong condE eval_always_result eval_rules.simps option.inject option.simps(3))
+  then show ?case sorry (*
+    by (simp add: eval_single_choice join_common_empty join_uncommon_empty)*)
+next
+  case (Cons a rules)
+  then show ?case sorry
+qed
+end
+
+
+lemmas monotonic =
+  monotonic_cond
+  monotonic_else
+  monotonic_choice
+  monotonic_seq
+
+lemma unordered_choice:
+  assumes "set rules = set rules'"
+  shows "\<forall>e. eval_rules (choice rules) u e = eval_rules (choice rules') u e"
+  using assms by (metis choiceE eval_choice_none eval_rules.intros(6))
+
+lemma find_inverse_lhs:
+  "\<exists>e. find_common m rules = None \<longleftrightarrow> find_uncommon m rules = Some e"
+  by (smt (verit, best) find_common.elims find_uncommon.simps(1) find_uncommon.simps(2) find_uncommon.simps(3) find_uncommon.simps(4) find_uncommon.simps(5))
+
+lemma find_inverse_rhs:
+  "\<exists>e. find_common m rules = Some e \<longleftrightarrow> find_uncommon m rules = None"
+  by (smt (verit, best) find_common.elims find_uncommon.simps(1) find_uncommon.simps(2) find_uncommon.simps(3) find_uncommon.simps(4) find_uncommon.simps(5))
+
+lemma join_common_equal:
+  assumes "find_common m a = None"
+  shows "(map ((?) m) (join_common m rules')) = (map ((?) m) (join_common m (a # rules')))"
+  apply (simp add: join_common_def join_uncommon_def List.map_filter_def)
+  by (simp add: assms)
+
+lemma join_common_plus:
+  assumes "find_common m a = Some a'"
+  shows "(m ? a') # (map ((?) m) (join_common m rules')) = (map ((?) m) (join_common m (a # rules')))"
+  using assms unfolding join_common_def join_uncommon_def List.map_filter_def
+  by simp
+
+experiment begin
+lemma pull_out_uncommon:
+  assumes "join_common m rules = []"
+  shows "eval_rules (choice (join_uncommon m rules)) u e = eval_rules (choice (rules)) u e"
+proof -
+  have "\<forall>r \<in> (set rules). find_common m r = None"
+    using assms unfolding join_common_def List.map_filter_def
+    by (simp add: filter_empty_conv)
+  then have "\<forall>r \<in> set rules. \<exists>p. find_uncommon m r = Some p"
+    using assms unfolding join_common_def join_uncommon_def List.map_filter_def
+    using find_inverse_lhs by blast
+  then have "rules = join_uncommon m rules"
+    unfolding join_common_def join_uncommon_def List.map_filter_def
+    by (smt (verit, ccfv_threshold) comp_eq_dest_lhs filter_id_conv find_uncommon_preserve map_idI option.sel option.simps(3))
+  then show ?thesis
+    by simp
+qed
+
+lemma pull_out_common:
+  assumes "join_uncommon m rules = []"
+  shows "eval_rules (m ? choice (r # join_common m rules)) u e = eval_rules (choice ((m ? r) # rules)) u e"
+  using assms sorry
+
+lemma pull_out:
+  shows "
+    eval_rules (choice ((m ? r) # rules)) u e =
+    eval_rules (choice ((m ? (choice (r # join_common m rules))) # [(choice (join_uncommon m rules))])) u e"
+  using pull_out_uncommon pull_out_common sorry
+
+lemma combine_conditions:
+  "eval_rules r u e = eval_rules (combine_conditions r) u e"
+  apply (induction r arbitrary: u e rule: combine_conditions.induct) apply simp
+  apply (simp add: monotonic)+
+        defer
+  apply simp+
+  apply (metis choice_join combine_conditions.simps(1) list.simps(9) monotonic_choice)
+  using monotonic_choice
+  using combine_conditions.simps(7) monotonic_choice apply presburger
+  using combine_conditions.simps(8) monotonic_choice apply presburger
+  using combine_conditions.simps(9) monotonic_choice apply presburger
+   apply (simp add: monotonic)+
+  using pull_out sorry
+
+end
+
+lemma join_combines:
+  "(set (map (\<lambda>r. m ? r) (join_common m rules)) \<union> set (join_uncommon m rules)) = set rules"
+  apply (induction rules) 
+    apply (simp add: join_common_def join_uncommon_def List.map_filter_def)
+  subgoal premises induct for a rules'
+  proof (cases "find_common m a")
+    case None
+    have "find_uncommon m a = Some a" 
+      using None find_inverse_lhs
+      by (metis find_uncommon_preserve option.distinct(1))
+    then have "join_uncommon m (a # rules') = a # (join_uncommon m rules')"
+      unfolding join_common_def join_uncommon_def List.map_filter_def
+      by simp
+    then show ?thesis using induct join_common_equal
+      by (metis None Un_insert_right list.simps(15))
+  next
+    case (Some a')
+    have "find_uncommon m a = None" 
+      by (metis Some find_common_defn find_uncommon.simps(1) option.distinct(1))
+    then have "join_uncommon m (a # rules') = (join_uncommon m rules')"
+      unfolding join_common_def join_uncommon_def List.map_filter_def
+      by simp
+    then show ?thesis
+      by (metis Some Un_insert_left find_common.elims induct join_common_plus list.simps(15) option.distinct(1))
+  qed
+  done
+
+experiment begin
+lemma abstract_combine_condition:
+  assumes "\<forall>u e. eval_rules (choice (r # ms)) u e \<longrightarrow> eval_rules (f (choice (r # ms))) u e"
+  assumes "\<forall>u e. eval_rules (choice n) u e \<longrightarrow> eval_rules (f (choice n)) u e"
+  assumes "(set (map (\<lambda>r. m ? r) ms) \<union> set n) = set rules"
+  shows "eval_rules (choice ((m ? r) # rules)) u e \<longrightarrow>
+       eval_rules
+        (choice
+          [m ? f (choice (r # ms)),
+           f (choice (n))]) u e"
+  using assms sorry
+
+lemma combine_conditions_lhs:
+  "eval_rules r u e = eval_rules (combine_conditions r) u e"
+  apply (induction r arbitrary: u e rule: combine_conditions.induct) apply simp
+  apply (simp add: monotonic)+
+        defer
+  apply simp+
+  apply (metis choice_join combine_conditions.simps(1) list.simps(9) monotonic_choice)
+  using monotonic_choice
+  using combine_conditions.simps(7) monotonic_choice apply presburger
+  using combine_conditions.simps(8) monotonic_choice apply presburger
+  using combine_conditions.simps(9) monotonic_choice apply presburger
+   apply (simp add: monotonic)+
+  sorry
+
+lemma
+  assumes "\<forall>u e. eval_rules (choice (r # join_common m rules)) u e \<longrightarrow>
+           eval_rules (combine_conditions (choice (r # join_common m rules))) u e"
+  assumes "\<forall>u e. eval_rules (choice (join_uncommon m rules)) u e \<longrightarrow>
+           eval_rules (combine_conditions (choice (join_uncommon m rules))) u e"
+  shows "eval_rules (choice ((m ? r) # rules)) u e \<longrightarrow>
+       eval_rules
+        (choice
+          [m ? combine_conditions (choice (r # join_common m rules)),
+           combine_conditions (choice (join_uncommon m rules))])
+        u e"
+  sorry
+
+lemma combine_nested:
+  assumes "set rules = {choice r} \<union> set r'"
+  assumes "set rules' = set r \<union> set r'"
+  shows "\<forall>e. eval_rules (choice rules) u e = eval_rules (choice rules') u e"
+  using assms
+proof -
+  obtain e' where "eval_rules (choice r) u e'"
+    using eval_always_result by auto
+  show ?thesis proof (cases e')
+    case None
+    have "\<forall>e. eval_rules (choice rules) u e = eval_rules (choice r') u e"
+      using choiceE assms sorry
+    then show ?thesis sorry
+  next
+    case (Some a)
+    then show ?thesis sorry
+  qed
+qed
+end
+
+lemma join_common_set_def:
+  "set (join_common m rules) = {r. (m ? r) \<in> set rules}"
+  unfolding join_common_def List.map_filter_def 
+  apply (induction rules)
+   apply simp 
+  subgoal for a rules 
+    apply (cases a) by auto
+  done
+
+lemma join_uncommon_set_def:
+  "set (join_uncommon m rules) = {r. r \<in> set rules \<and> (\<forall>r'. r \<noteq> (m ? r'))}"
+  unfolding join_uncommon_def List.map_filter_def 
+  apply (induction rules) apply simp
+  subgoal for a rules 
+    apply (cases a) by auto
+  done
+
+experiment begin
+lemma idempotent_match:
+  assumes "valid_match m"
+  assumes "eval_match m u = Some r"
+  shows "eval_match m r = Some r"
+  using assms sorry (*
+  by (metis eval_match.simps(6) match_eq option.simps(5))*)
+end
+
+lemma
+  assumes "\<exists>r \<in> set rules. r \<in> set rules' \<and> eval_rules r u (Some e)"
+  shows "eval_rules (choice rules) u (Some e) = eval_rules (choice rules') u (Some e)"
+  using assms
+  using eval_rules.intros(6) by blast
+
+lemma map_None:
+  "(\<forall>r\<in>set rules. eval_rules (m ? r) u None) = eval_rules (choice (map ((?) m) rules)) u None"
+  (is "?lhs = eval_rules ?rhs u None")
+proof -
+  have setequiv: "set (map ((?) m) rules) = {m ? r | r . r\<in>set rules}"
+    by (simp add: Setcompr_eq_image)
+  then show ?thesis
+    using eval_choice_none by auto
+qed
+
+lemma setequiv: "set (map ((?) m) rules) = {m ? r | r . r\<in>set rules}"
+  by (simp add: Setcompr_eq_image)
+
+lemma pull_cond_out_rhs:
+  assumes "eval_rules (choice (map ((?) m) rules)) u e" (is "eval_rules ?lhs u e")
+  shows "eval_rules (m ? choice rules) u e" (is "eval_rules ?rhs u e")
+  proof (cases "eval_match m u")
+    case None \<comment> \<open>If m doesn't match then both the lhs and rhs should evaluate to e = None\<close>
+    have lhs: "\<forall>e. eval_rules ?lhs u e \<longrightarrow> e = None"
+      using None eval_rules.intros(3) eval_rules.intros(7)
+      by (smt (verit, del_insts) choiceE condE ex_map_conv option.distinct(1))
+    have rhs: "\<forall>e. eval_rules ?rhs u e \<longrightarrow> e = None"
+      by (metis None condE option.distinct(1))
+    then show ?thesis using lhs rhs
+      using eval_always_result
+      using assms by blast
+  next
+    case match: (Some a) \<comment> \<open>Drop down into evaluation post matching m\<close>
+      have allEval: "\<forall>r \<in> set rules. eval_rules r a e = eval_rules (m ? r) u e"
+        by (metis match condE eval_rules.intros(2) option.distinct(1) option.sel)
+        then show ?thesis
+        proof (cases e)
+          case evalsNone: None
+          have "\<forall>r \<in> set rules. eval_rules r a None"
+            using evalsNone allEval assms map_None by blast
+          then have "\<forall>r \<in> set rules. eval_rules (m ? r) u None"
+            using evalsNone allEval by blast
+          then have "eval_rules ?lhs u None"
+            by (simp add: map_None)
+          then show ?thesis
+            using evalsNone
+            using \<open>\<forall>r\<in>set rules. eval_rules r a None\<close> eval_choice_none eval_rules.intros(2) match by blast
+        next
+          case evalsSome: (Some a')
+            then have "\<exists>r \<in> set rules. eval_rules (m ? r) u (Some a')"
+              using condE assms match
+              using choiceE by fastforce
+            then have "\<exists>r \<in> set rules. eval_rules (m ? r) u e"
+              by (simp add: evalsSome)
+            then have "eval_rules ?rhs u e"
+              using allEval eval_rules.intros(2) eval_rules.intros(6) evalsSome match by blast
+            then show ?thesis
+              by simp
+          qed
+        qed
+
+lemma pull_cond_out_lhs:
+  assumes "eval_rules (m ? choice rules) u e" (is "eval_rules ?lhs u e")
+  shows "eval_rules (choice (map ((?) m) rules)) u e" (is "eval_rules ?rhs u e")
+  proof (cases "eval_match m u")
+    case None \<comment> \<open>If m doesn't match then both the lhs and rhs should evaluate to e = None\<close>
+    have lhs: "\<forall>e. eval_rules ?lhs u e \<longrightarrow> e = None"
+      using None eval_rules.intros(3) eval_rules.intros(7)
+      by (smt (verit, del_insts) choiceE condE ex_map_conv option.distinct(1))
+    have rhs: "\<forall>e. eval_rules ?rhs u e \<longrightarrow> e = None"
+      by (simp add: lhs pull_cond_out_rhs)
+    then show ?thesis using lhs rhs
+      using eval_always_result
+      using assms by blast
+  next
+    case match: (Some a) \<comment> \<open>Drop down into evaluation post matching m\<close>
+      have allEval: "\<forall>r \<in> set rules. eval_rules r a e = eval_rules (m ? r) u e"
+        by (metis match condE eval_rules.intros(2) option.distinct(1) option.sel)
+        then show ?thesis
+        proof (cases e)
+          case evalsNone: None
+          have "\<forall>r \<in> set rules. eval_rules r a None"
+            by (metis assms condE eval_choice_none evalsNone match option.discI option.inject)
+          then have "\<forall>r \<in> set rules. eval_rules (m ? r) u None"
+            using evalsNone allEval by blast
+          then show ?thesis
+            using evalsNone map_None by blast
+        next
+          case evalsSome: (Some a')
+            then have "\<exists>r \<in> set rules. eval_rules (m ? r) u (Some a')"
+              using condE assms match
+              using choiceE
+              by (metis allEval option.distinct(1) option.sel)
+            then have "\<exists>r \<in> set rules. eval_rules (m ? r) u e"
+              by (simp add: evalsSome)
+            then have "eval_rules ?rhs u e"
+              by (metis eval_rules.intros(6) evalsSome image_eqI image_set)
+            then show ?thesis
+              by simp
+          qed
+        qed
+
+lemma pull_cond_out:
+  "eval_rules (choice (map ((?) m) rules)) u e = eval_rules (m ? choice rules) u e"
+  using pull_cond_out_lhs pull_cond_out_rhs by blast
+
+lemma cases_None:
+  assumes "eval_rules (choice ((m ? r) # rules)) u None"
+  shows "
+  eval_rules (m ? (choice (r # join_common m rules))) u None \<and>
+  eval_rules ((choice (join_uncommon m rules))) u None"
+  apply (rule conjI)
+  using assms
+  unfolding join_common_def List.map_filter_def
+   apply (induction rules) apply simp using pull_cond_out
+    apply fastforce apply auto[1] using pull_cond_out defer defer
+    apply (meson assms eval_choice_none join_uncommon_subset list.set_intros(2) subsetD)
+  subgoal for a rules y
+    apply (cases a)
+        apply force
+    subgoal premises pre for m' r' 
+    proof -
+      have "m = m'"
+        using pre(3,4)
+        by (metis find_common.simps(1) option.distinct(1))
+      then show ?thesis using pre apply auto
+        by (smt (verit, del_insts) eval_choice_none list.set_intros(1) list.set_intros(2) list.simps(9) pull_cond_out set_ConsD)
+    qed
+      by simp+
+  subgoal for a rules
+    apply (cases a)
+    by (simp add: eval_choice_none)+
+  done
+
+lemma cases_None1:
+  assumes "
+  eval_rules (m ? (choice (r # join_common m rules))) u None \<and>
+  eval_rules ((choice (join_uncommon m rules))) u None"
+  shows "eval_rules (choice ((m ? r) # rules)) u None"
+proof -
+  have head: "eval_rules (m ? r) u None"
+    using assms
+    by (meson list.set_intros(1) map_None pull_cond_out_lhs)
+  have common_None: "\<forall>r' \<in> set (join_common m rules). eval_rules (m ? r') u None"
+    by (meson assms list.set_intros(2) map_None pull_cond_out_lhs)
+  have uncommon_None: "\<forall>r' \<in> set (join_uncommon m rules). eval_rules r' u None"
+    using assms eval_choice_none by blast
+  have "\<forall>r' \<in> set rules. eval_rules r' u None"
+    using join_combines common_None uncommon_None pull_cond_out
+    by (metis (no_types, lifting) UnE assms eval_choice_none list.set_intros(2) list.simps(9))
+  then show ?thesis using head
+    by (simp add: eval_choice_none)
+qed
+
+  
+lemma cases_Some:
+  assumes "eval_rules (choice rules) u (Some e)"
+  shows "
+  eval_rules (m ? (choice (join_common m rules))) u (Some e) \<or>
+  eval_rules ((choice (join_uncommon m rules))) u (Some e)"
+proof -
+  obtain r where r: "r \<in> set rules \<and> eval_rules r u (Some e)"
+    by (metis assms choiceE option.discI)
+  then show ?thesis
+  proof (cases r)
+    case (base x1)
+    have "r \<in> set (join_uncommon m rules)"
+      using join_uncommon_set_def base r by blast
+    then show ?thesis
+      using eval_rules.intros(6) r by presburger
+  next
+    case (cond m' r')
+    then show ?thesis
+    proof (cases "m = m'")
+      case True
+      then have "r' \<in> set (join_common m rules)"
+        using cond r join_common_set_def
+        by blast
+      then show ?thesis
+        by (metis True cond eval_rules.intros(6) image_eqI image_set pull_cond_out_rhs r)
+    next
+      case False
+      have "r \<in> set (join_uncommon m rules)"
+        using join_uncommon_set_def False r
+        using cond by blast
+      then show ?thesis
+        using eval_rules.intros(6) r by presburger
+    qed
+  next
+    case (else x31 x32)
+    have "r \<in> set (join_uncommon m rules)"
+      using join_uncommon_set_def else r by blast
+    then show ?thesis
+      using eval_rules.intros(6) r by presburger
+  next
+    case (seq x41 x42)
+    have "r \<in> set (join_uncommon m rules)"
+      using join_uncommon_set_def seq r by blast
+    then show ?thesis
+      using eval_rules.intros(6) r by presburger
+  next
+    case (choice x5)
+    have "r \<in> set (join_uncommon m rules)"
+      using join_uncommon_set_def choice r by blast
+    then show ?thesis
+      using eval_rules.intros(6) r by presburger
+  qed
+qed
+
+lemma cases_Some1:
+  assumes "eval_rules (choice ((m ? r) # rules)) u (Some e)"
+  shows "
+  eval_rules (m ? (choice (r # join_common m rules))) u (Some e) \<or>
+  eval_rules ((choice (join_uncommon m rules))) u (Some e)"
+  using cases_Some assms
+  by (smt (verit, ccfv_threshold) choiceE eval_rules.intros(6) list.set_intros(1) list.set_intros(2) list.simps(9) option.distinct(1) pull_cond_out set_ConsD)
+
+lemma cases_Some2:
+  assumes "eval_rules (m ? (choice (r # join_common m rules))) u (Some e) \<or>
+  eval_rules ((choice (join_uncommon m rules))) u (Some e)" (is "?c1 \<or> ?c2")
+  shows "eval_rules (choice ((m ? r) # rules)) u (Some e)"
+using assms proof (rule disjE)
+  assume c1: "?c1"
+  then show ?thesis
+  proof (cases "eval_rules (m ? r) u (Some e)")
+    case True
+    then show ?thesis
+      by (meson eval_rules.intros(6) list.set_intros(1))
+  next
+    case False
+    then have "\<exists>r \<in>set (join_common m rules). eval_rules (m ? r) u (Some e)"
+      using c1
+      by (smt (verit, del_insts) choiceE condE eval_rules.intros(2) option.distinct(1) set_ConsD)
+    then show ?thesis 
+      by (metis eval_rules.intros(6) join_common_set_def list.set_intros(2) mem_Collect_eq)
+  qed
+next
+  assume "?c2"
+  then have "\<exists>r \<in>set (join_uncommon m rules). eval_rules r u (Some e)"
+    by (metis choiceE option.discI)
+  then show ?thesis
+    by (meson eval_rules.intros(6) join_uncommon_subset list.set_intros(2) subsetD)
+qed
+
+lemma evalchoice_twoelement:
+  assumes "eval_rules (choice [x1, x2]) u (Some e)"
+  shows "eval_rules x1 u (Some e) \<or> eval_rules x2 u (Some e)"
+  using assms choiceE by fastforce
+
+lemma combine_conditions_valid:
+  "eval_rules r u e = eval_rules (combine_conditions r) u e"
+  apply (induction r arbitrary: u e rule: combine_conditions.induct) apply simp
+  apply (simp add: monotonic)+
+        defer
+  apply simp+
+  apply (metis choice_join combine_conditions.simps(1) list.simps(9) monotonic_choice)
+  using monotonic_choice
+  using combine_conditions.simps(7) monotonic_choice apply presburger
+  using combine_conditions.simps(8) monotonic_choice apply presburger
+  using combine_conditions.simps(9) monotonic_choice apply presburger
+   apply (simp add: monotonic)+
+  subgoal premises p for m r rules u e
+  proof (rule iffI)
+    assume eval: "eval_rules (choice ((m ? r) # rules)) u e"
+    show "eval_rules
+     (choice
+       [m ? combine_conditions (choice (r # join_common m rules)),
+        combine_conditions (choice (join_uncommon m rules))])
+     u e"
+    proof (cases e)
+      case None
+      have "eval_rules (m ? (choice (r # join_common m rules))) u None \<and>
+  eval_rules ((choice (join_uncommon m rules))) u None"
+        using None cases_None eval by blast
+      then have "eval_rules (m ? combine_conditions (choice (r # join_common m rules))) u None \<and>
+  eval_rules (combine_conditions (choice (join_uncommon m rules))) u None" 
+        using p monotonic_cond by blast
+      then show ?thesis using None eval_choice_none by simp
+    next
+      case (Some a)
+      have "eval_rules (m ? (choice (r # join_common m rules))) u (Some a) \<or>
+  eval_rules ((choice (join_uncommon m rules))) u (Some a)"
+        using Some cases_Some1 eval by simp
+      then have "eval_rules (m ? combine_conditions (choice (r # join_common m rules))) u (Some a) \<or>
+  eval_rules (combine_conditions (choice (join_uncommon m rules))) u (Some a)"
+        using p monotonic_cond by blast
+      then show ?thesis
+        by (metis Some eval_rules.intros(6) list.set_intros(1) list.set_intros(2))
+    qed
+  next
+    assume eval: "eval_rules
+     (choice
+       [m ? combine_conditions (choice (r # join_common m rules)),
+        combine_conditions (choice (join_uncommon m rules))])
+     u e"
+    show "eval_rules (choice ((m ? r) # rules)) u e"
+    proof (cases e)
+      case None
+      then have "eval_rules (m ? (choice (r # join_common m rules))) u None \<and>
+  eval_rules ((choice (join_uncommon m rules))) u None"
+        by (smt (verit) eval eval_choice_none list.set_intros(1) list.set_intros(2) monotonic_cond p(1) p(2))
+      then show ?thesis using cases_None1 None by blast
+    next
+      case (Some a)
+      then have "eval_rules (m ? combine_conditions (choice (r # join_common m rules))) u (Some a) \<or>
+  eval_rules (combine_conditions (choice (join_uncommon m rules))) u (Some a)"
+        using eval evalchoice_twoelement by simp
+      then have "eval_rules (m ? (choice (r # join_common m rules))) u (Some a) \<or>
+  eval_rules ((choice (join_uncommon m rules))) u (Some a)"
+        using p monotonic_cond by blast
+      then show ?thesis using cases_Some2 Some
+        by simp
+    qed
+  qed
+  done
+
+(*
+  proof (cases e)
+    case None
+    then have "eval_rules (m ? (choice (r # join_common m rules))) u None \<and>
+  eval_rules ((choice (join_uncommon m rules))) u None"
+      sorry
+    then show ?thesis using p sorry
+  next
+    case (Some a)
+    then show ?thesis sorry
+  qed*)
+
+(*
+  proof (cases e)
+    case None
+    then show ?thesis 
+      apply simp apply (rule choiceE) using None cases_None
+      using eval_always_result apply auto
+  next
+    case (Some a)
+    then show ?thesis sorry
+  qed
+
+  using join_combines unordered_choice monotonic_choice combine_nested
+  
+  done
+*)
+
+(*
+lemma combine_conditions_valid:
+  "{e. eval_rules r u e} = {e. eval_rules (combine_conditions r) u e}"
+  apply (induction r arbitrary: u rule: combine_conditions.induct)
+  apply simp unfolding combine_conditions.simps
+  apply (smt (verit, del_insts) Collect_cong elseE eval_rules.intros(4) eval_rules.intros(5) mem_Collect_eq)
+  unfolding combine_conditions.simps 
+  apply (smt (z3) Collect_cong condE eval_rules.simps mem_Collect_eq)
+  unfolding combine_conditions.simps 
+  subgoal for m r rules u
+    using combine_no_recurse sorry
+  sorry*)
+    (*apply (smt (verit, del_insts) elseE eval_rules.intros(4) eval_rules.intros(5) lift_common.simps(1) option.simps(4))
+      by (simp add: join_conditions_valid)
+    subgoal for m r u apply (cases "join_conditions (m ? r)")
+       apply simp apply (metis condE eval_rules.intros(2) eval_rules.intros(3))
+      by (simp add: join_conditions_valid)
+    subgoal for rules u apply (induction rules)
+      apply simp
+      by (metis choice_join lift_common.simps(3) list.set_intros(1) list.set_intros(2))
+     apply simp
+    by (smt (verit) Rules.distinct(11) Rules.distinct(15) Rules.distinct(19) Rules.distinct(5) Rules.inject(4) eval_rules.simps lift_common.simps(5))
+*)
+
+fun eliminate_choice :: "Rules \<Rightarrow> Rules" where
+  "eliminate_choice (base e) = base e" |
+  "eliminate_choice (r1 else r2) = (eliminate_choice r1 else eliminate_choice r2)" |
+  "eliminate_choice (m ? r) = (m ? eliminate_choice r)" |
+  "eliminate_choice (choice (r # [])) = eliminate_choice r" |
+  "eliminate_choice (choice rules) = 
+    choice (map eliminate_choice rules)" |
+  "eliminate_choice (r1 \<then> r2) = (eliminate_choice r1 \<then> eliminate_choice r2)"
+
+lemma choice_Single:
+  "eval_rules (choice [r]) u e = eval_rules r u e"
+  apply (cases e)
+  using eval_choice_none apply auto[1]
+  using choiceE eval_rules.intros(6) by fastforce
+
+lemma eliminate_choice_valid:
+  "{e. eval_rules r u e} = {e. eval_rules (eliminate_choice r) u e}"
+  apply (induction r arbitrary: u rule: eliminate_choice.induct)
+  apply simp unfolding eliminate_choice.simps
+  apply (smt (verit) Collect_cong elseE eval_rules.intros(4) eval_rules.intros(5) mem_Collect_eq)
+  unfolding eliminate_choice.simps
+      apply (smt (verit) Collect_cong condE eval_rules.intros(3) eval_rules.simps mem_Collect_eq)
+  unfolding eliminate_choice.simps
+  using choice_Single apply presburger
+  using monotonic_choice apply blast
+  apply (metis Collect_cong mem_Collect_eq monotonic_choice)
+  by (smt (verit) Collect_cong eval_rules.intros(10) eval_rules.intros(9) mem_Collect_eq seqE)
+
+
+(*definition optimized_export where
+  "optimized_export = eliminate_choice o combine_conditions o lift_common o lift_match o eliminate_noop o eliminate_empty"
 *)
 
 definition optimized_export where
-  "optimized_export = lift_common o lift_match o eliminate_noop o eliminate_empty"
+  "optimized_export = eliminate_choice o combine_conditions o lift_match o eliminate_noop o eliminate_empty"
+
 
 lemma optimized_export_valid:
-  "eval_rules r u e = eval_rules (optimized_export r) u e"
+  "{e. eval_rules r u e} = {e. eval_rules (optimized_export r) u e}"
   unfolding optimized_export_def comp_def
-  using lift_common_valid lift_match_valid eliminate_noop_valid eliminate_empty_valid by simp
+  using lift_match_valid eliminate_noop_valid eliminate_empty_valid 
+  using combine_conditions_valid eliminate_choice_valid by simp
+
+thm_oracles optimized_export_valid
+
+
+subsection \<open>Java AST\<close>
+
+type_synonym ClassName = string
+type_synonym VariableName = String.literal
+type_synonym MethodName = string
+
+datatype Expression =
+  Ref VariableName |
+  IntegerConstant int |
+  TrueValue |
+  FalseValue |
+  MethodCall Expression MethodName "Expression list" |
+  Constructor ClassName "Expression list" |
+  InstanceOf Expression ClassName VariableName |
+  Equal Expression Expression |
+  Less Expression Expression |
+  Negate Expression |
+  And Expression Expression |
+  BitAnd Expression Expression |
+  Unsupported string
+
+datatype Statement =
+  Assignment VariableName Expression |
+  Branch Expression Statement |
+  Return Expression |
+  Sequential "Statement list"
+
+fun intersperse :: "string \<Rightarrow> string list \<Rightarrow> string list" where
+  "intersperse i es = foldr (\<lambda>x ys . x # (if ys = [] then ys else i # ys)) es []"
+
+fun param_list :: "string list \<Rightarrow> string" where
+  "param_list es = (foldr (@) (intersperse '', '' es) '''')"
+
+fun generate_expression :: "Expression \<Rightarrow> string" where
+  "generate_expression (Ref v) = String.explode v" |
+  "generate_expression (IntegerConstant n) = ''0''" | (*TODO FIX*)
+  "generate_expression TrueValue = ''true''" |
+  "generate_expression FalseValue = ''false''" |
+  "generate_expression (MethodCall e mn ps) = 
+    (generate_expression e) @ ''.'' @ mn @ ''('' @ param_list (map generate_expression ps) @ '')''" |
+  "generate_expression (Constructor cn ps) =
+    ''new '' @ cn @ ''('' @ param_list (map generate_expression ps) @ '')''" |
+  "generate_expression (InstanceOf e cn var) =
+    (generate_expression e) @ '' instanceof '' @ cn @ '' '' @ (String.explode var)" |
+  "generate_expression (Equal e1 e2) =
+    (generate_expression e1) @ '' == '' @ (generate_expression e2)" |
+  "generate_expression (Less e1 e2) =
+    (generate_expression e1) @ '' < '' @ (generate_expression e2)" |
+  "generate_expression (Negate e) =
+    ''!('' @ (generate_expression e) @ '')''" |
+  "generate_expression (And e1 e2) =
+    (generate_expression e1) @ '' && '' @ (generate_expression e2)" |
+  "generate_expression (BitAnd e1 e2) =
+    (generate_expression e1) @ '' & '' @ (generate_expression e2)"
+
+fun indent :: "nat \<Rightarrow> string" where
+  "indent 0 = ''''" |
+  "indent (Suc n) = '' '' @ indent n"
+
+fun generate_statement :: "nat \<Rightarrow> Statement \<Rightarrow> string" where
+  "generate_statement i (Assignment v e) = indent i @
+    ''var '' @ String.explode v @ '' = '' @ generate_expression e @ '';\<newline>''" |
+  "generate_statement i (Branch c s) = indent i @
+    ''if ('' @ generate_expression c @ '') {\<newline>'' @ generate_statement (i + 4) s @ 
+    indent i @ ''}\<newline>''" |
+  "generate_statement i (Return e) = indent i @
+    ''return '' @ generate_expression e @ '';\<newline>''" |
+  "generate_statement i (Sequential ss) = 
+    foldr (@) (map (generate_statement i) ss) ''''"
 
 
 subsection \<open>Java Generation\<close>
 
-fun unary_op_class :: "IRUnaryOp \<Rightarrow> string" where
+fun unary_op_class :: "IRUnaryOp \<Rightarrow> ClassName" where
   "unary_op_class UnaryAbs = ''AbsNode''" |
-  "unary_op_class UnaryNeg = ''NegNode''" |
+  "unary_op_class UnaryNeg = ''NegateNode''" |
   "unary_op_class UnaryNot = ''NotNode''" |
   "unary_op_class UnaryLogicNegation = ''LogicNegationNode''" |
   "unary_op_class (UnaryNarrow _ _) = ''NarrowNode''" |
   "unary_op_class (UnarySignExtend _ _) = ''SignExtendNode''" |
   "unary_op_class (UnaryZeroExtend _ _) = ''ZeroExtendNode''"
 
-fun binary_op_class :: "IRBinaryOp \<Rightarrow> string" where
+fun binary_op_class :: "IRBinaryOp \<Rightarrow> ClassName" where
   "binary_op_class BinAdd = ''AddNode''" |
   "binary_op_class BinMul = ''MulNode''" |
   "binary_op_class BinSub = ''SubNode''" |
@@ -982,7 +2344,7 @@ fun binary_op_class :: "IRBinaryOp \<Rightarrow> string" where
   "binary_op_class BinIntegerLessThan = ''IntegerLessThanNode''" |
   "binary_op_class BinIntegerBelow = ''IntegerBelowNode''"
 
-fun export_pattern :: "PatternExpr \<Rightarrow> string" where
+fun export_pattern :: "PatternExpr \<Rightarrow> ClassName" where
   "export_pattern (UnaryPattern op v) = unary_op_class op" |
   "export_pattern (BinaryPattern op v1 v2) = binary_op_class op" |
   "export_pattern (ConditionalPattern v1 v2 v3) = ''ConditionalNode''" |
@@ -999,67 +2361,105 @@ definition string_of_int :: "int \<Rightarrow> string" where
   "string_of_int i = (if i < 0 then ''-'' @ string_of_nat (nat (- i)) else 
      string_of_nat (nat i))"
 
-fun export_value :: "Value \<Rightarrow> string" where
-  "export_value (IntVal s v) = string_of_int (sint v)" |
-  "export_value _ = ''ERROR: unsupported Value''"
+fun export_value :: "Value \<Rightarrow> Expression" where
+  "export_value (IntVal s v) = IntegerConstant (sint v)" |
+  "export_value _ = Unsupported ''unsupported Value''"
 
-fun export_assignments :: "VarName \<Rightarrow> PatternExpr \<Rightarrow> string" where
-  "export_assignments v (UnaryPattern op v1) = 
-    ''var '' @ String.explode v1 @ '' = '' @ String.explode v @ ''.getX();
-''" |
-  "export_assignments v (BinaryPattern op v1 v2) = 
-    ''var '' @ String.explode v1 @ '' = '' @ String.explode v @ ''.getX();
-var '' @ String.explode v2 @ '' = '' @ String.explode v @ ''.getY();
-''" |
-  "export_assignments v (ConditionalPattern v1 v2 v3) =
-    ''var '' @ String.explode v1 @ '' = '' @ String.explode v @ ''.condition();
-var '' @ String.explode v2 @ '' = '' @ String.explode v @ ''.trueValue();
-var '' @ String.explode v3 @ '' = '' @ String.explode v @ ''.falseValue();
-''" |
-  "export_assignments v (ConstantPattern val) =
-    ''if ('' @ String.explode v @ ''.getValue() == '' @ export_value val @ '') {''" |
-  "export_assignments v (ConstantVarPattern var) =
-    ''if ('' @ String.explode v @ ''.getValue() == '' @ String.explode var @ '') {''"
-
-fun export_irexpr :: "IRExpr \<Rightarrow> string" where
+fun export_irexpr :: "IRExpr \<Rightarrow> Expression" where
   "export_irexpr (UnaryExpr op e1) =
-    ''new '' @ unary_op_class op @ ''('' @ export_irexpr e1 @ '')''" |
+    Constructor (unary_op_class op) [export_irexpr e1]" |
   "export_irexpr (BinaryExpr op e1 e2) =
-    ''new '' @ binary_op_class op @ ''('' @ export_irexpr e1 @ '', '' @ export_irexpr e2 @ '')''" |
+    Constructor (binary_op_class op) [export_irexpr e1, export_irexpr e2]" |
   "export_irexpr (ConditionalExpr e1 e2 e3) =
-    ''new ConditionalNode('' @ export_irexpr e1 @ '', '' @ export_irexpr e2 @ '', '' @ export_irexpr e3 @ '')''" |
+    Constructor ''ConditionalNode''  [export_irexpr e1, export_irexpr e2, export_irexpr e3]" |
   "export_irexpr (ConstantExpr val) =
-    ''new ConstantNode('' @ export_value val @ '')''" |
+    Constructor ''ConstantNode'' [export_value val]" |
   "export_irexpr (ConstantVar var) =
-    ''new ConstantNode('' @ String.explode var @ '')''" |
-  "export_irexpr (VariableExpr v s) = String.explode v"
+    Constructor ''ConstantNode'' [Ref var]" |
+  "export_irexpr (VariableExpr v s) = Ref v"
 
-fun export_condition :: "SideCondition \<Rightarrow> string" where
-  "export_condition (IsConstantExpr e) = export_irexpr e @ '' instanceof ConstantNode''" |
-  "export_condition (WellFormed s) = ''true''" |
-  "export_condition (IsStamp e s) = export_irexpr e @ ''.stamp() == v''" |
-  "export_condition (StampUnder e1 e2) = ''stamp under''" |
-  "export_condition (UpMaskEquals e m) = ''up mask equals''" |
-  "export_condition (DownMaskEquals e m) = ''down mask equals''" |
-  "export_condition (UpMaskCancels e1 e2) = ''('' @ export_irexpr e1 @ ''.stamp().upMask() && '' @ export_irexpr e2 @ ''.stamp().upMask()) == 0''" |
-  "export_condition (Not sc) = ''!('' @ export_condition sc @ '')''" |
-  "export_condition (And sc1 sc2) = ''('' @ export_condition sc1 @ '') && ('' @ export_condition sc2 @ '')''" |
-  "export_condition (Empty) = ''true''"
+fun export_stamp :: "Stamp \<Rightarrow> Expression" where
+  "export_stamp (IntegerStamp bits lower higher) =
+    Constructor ''IntegerStamp'' 
+      [IntegerConstant bits, IntegerConstant lower,
+       IntegerConstant higher]" |
+  "export_stamp _ =
+    Unsupported ''unsupported Stamp''"
 
-fun export_match :: "MATCH \<Rightarrow> string" where
-  "export_match (match v p) = ''if ('' @ String.explode v @ '' instanceof '' @ export_pattern p @ '') {
-'' @ export_assignments v p" |
-  "export_match (andthen m1 m2) = export_match m1 @ '''' @ export_match m2" |
-  "export_match (equality v1 v2) = ''if ('' @ String.explode v1 @ '' == '' @ String.explode v2 @ '') {
-''" |
-  "export_match (negate sc) = ''if (!('' @ export_condition sc @ '')) {
-''" |
-  "export_match (check sc) = ''if ('' @ export_condition sc @ '') {
-''" |
-  "export_match noop = ''''"
+definition stampOf :: "Expression \<Rightarrow> Expression" where
+  "stampOf e = (MethodCall e ''stamp'' [Ref STR ''view''])"
 
+definition upMask :: "Expression \<Rightarrow> Expression" where
+  "upMask e = (MethodCall (stampOf e) ''upMask'' [])"
 
+definition downMask :: "Expression \<Rightarrow> Expression" where
+  "downMask e = (MethodCall (stampOf e) ''downMask'' [])"
 
+fun export_condition :: "SideCondition \<Rightarrow> Expression" where
+  "export_condition (IsConstantExpr e) = (InstanceOf (export_irexpr e) ''ConstantNode'' STR ''t'')" |
+  "export_condition (WellFormed s) = TrueValue" |
+  "export_condition (IsStamp e s) =
+    (Equal (stampOf (export_irexpr e)) (export_stamp s))" |
+  "export_condition (StampUnder e1 e2) =
+    (Less 
+      (MethodCall (stampOf (export_irexpr e1)) ''upperBound'' []) 
+      (MethodCall (stampOf (export_irexpr e2)) ''lowerBound'' []))" |
+  "export_condition (UpMaskEquals e m) =
+    Equal (upMask (export_irexpr e)) (IntegerConstant (sint m))" |
+  "export_condition (DownMaskEquals e m) =
+    Equal (downMask (export_irexpr e)) (IntegerConstant (sint m))" |
+  "export_condition (UpMaskCancels e1 e2) =
+    Equal (BitAnd (upMask (export_irexpr e1)) (upMask (export_irexpr e2))) (IntegerConstant 0)" |
+  "export_condition (PowerOf2 e) =
+    MethodCall (Ref STR ''CodeUtil'') ''isPowerOf2'' [export_irexpr e]" |
+  "export_condition (IsBool e) =
+    Equal (MethodCall (export_irexpr e) ''upMask'' []) (IntegerConstant 1)" |
+  "export_condition (Not sc) = Negate (export_condition sc)" |
+  "export_condition (SideCondition.And sc1 sc2) = And (export_condition sc1) (export_condition sc2)" |
+  "export_condition (Empty) = TrueValue"
+
+fun export_assignments :: "VarName \<Rightarrow> PatternExpr \<Rightarrow> Statement \<Rightarrow> Statement" where
+  "export_assignments v (UnaryPattern op v1) s = Sequential
+    [Assignment v1 (MethodCall (Ref (v + STR ''c'')) ''getValue'' []), s]" |
+  "export_assignments v (BinaryPattern op v1 v2) s = Sequential
+    [Assignment v1 (MethodCall (Ref (v + STR ''c'')) ''getX'' []),
+     Assignment v2 (MethodCall (Ref (v + STR ''c'')) ''getY'' []), s]" |
+  "export_assignments v (ConditionalPattern v1 v2 v3) s = Sequential
+    [Assignment v1 (MethodCall (Ref (v + STR ''c'')) ''condition'' []),
+     Assignment v2 (MethodCall (Ref (v + STR ''c'')) ''trueValue'' []),
+     Assignment v3 (MethodCall (Ref (v + STR ''c'')) ''falseValue'' []), s]" |
+  "export_assignments v (ConstantPattern val) s =
+    Branch (InstanceOf (MethodCall (Ref (v + STR ''c'')) ''getValue'' []) ''PrimitiveConstant'' (v + STR ''cd''))
+    (Branch (Equal (MethodCall (Ref (v + STR ''cd'')) ''asLong'' []) (export_value val)) s)" |
+  "export_assignments v (ConstantVarPattern var) s =
+    Branch (Equal (MethodCall (Ref (v + STR ''c'')) ''getValue'' []) (Ref var)) s"
+
+function (sequential) export_match :: "MATCH \<Rightarrow> Statement \<Rightarrow> Statement" where
+  "export_match (match v p) r  = 
+    Branch (InstanceOf (Ref v) (export_pattern p) (String.implode (String.explode v @ ''c'')))
+      (export_assignments v p r)" |
+  "export_match (andthen m1 m2) r = 
+    export_match m1 (export_match m2 r)" |
+  "export_match (equality v1 v2) r = 
+    Branch (Equal (Ref v1) (Ref v2)) r" |
+  "export_match (condition (SideCondition.And sc1 sc2)) r = 
+    Branch (export_condition sc1) (Branch (export_condition sc2) r)" |
+  "export_match (condition (WellFormed s)) r = r" |
+  "export_match (condition (Empty)) r = r" |
+  "export_match (condition sc) r = 
+    Branch (export_condition sc) r" |
+  "export_match noop r = r"
+  apply pat_completeness+
+  by simp+
+
+fun size_condition :: "(MATCH \<times> Statement) \<Rightarrow> nat" where
+  "size_condition ((condition c), s) = size (condition c) + size c" |
+  "size_condition (m, s) = size m"
+
+termination export_match
+  apply (relation "measures [size_condition]") apply simp apply simp sorry
+
+(*
 fun close :: "MATCH \<Rightarrow> string" where
   "close (match v (ConstantPattern val)) = ''
 }
@@ -1071,17 +2471,18 @@ fun close :: "MATCH \<Rightarrow> string" where
 }''" |
   "close (negate sc) = ''
 }''" |
-  "close (check sc) = ''
+  "close (condition sc) = ''
 }''" |
   "close noop = ''''"
+*)
 
-fun export_rules :: "Rules \<Rightarrow> string" where
-  "export_rules (base e) = ''return '' @ export_irexpr e @ '';''" |
-  "export_rules (cond m r) = export_match m @ export_rules r @ close m" |
-  "export_rules (r1 else r2) = export_rules r1 @ ''
-'' @ export_rules r2" |
-  "export_rules (r1 \<then> r2) = export_rules r1 @ ''
-'' @ export_rules r2" (* TODO: should modify e *)
+fun export_rules :: "Rules \<Rightarrow> Statement" where
+  "export_rules (base e) = Return (export_irexpr e)" |
+  "export_rules (cond m r) = export_match m (export_rules r)" |
+  "export_rules (r1 else r2) = Sequential [export_rules r1, export_rules r2]" |
+  "export_rules (choice rules) = Sequential (map export_rules rules)" |
+  "export_rules (r1 \<then> r2) = Sequential [export_rules r1, export_rules r2]" (* TODO: should modify e *)
+
 
 subsection \<open>Experiments\<close>
 
@@ -1118,7 +2519,7 @@ definition AddLeftNegateToSub where
 corollary
   "NestedNot =
    (MATCH.match STR ''e'' (UnaryPattern UnaryNot STR ''a'') &&
-    (MATCH.match STR ''a'' (UnaryPattern UnaryNot STR ''az'') && noop) && check Empty) ?
+    (MATCH.match STR ''a'' (UnaryPattern UnaryNot STR ''az'') && noop) && condition Empty) ?
       base (VariableExpr STR ''az'' VoidStamp)"
   by eval
 
@@ -1126,14 +2527,14 @@ corollary
   "RedundantSub =
    (MATCH.match STR ''e'' (BinaryPattern BinAdd STR ''a'' STR ''b'') &&
     (MATCH.match STR ''a'' (BinaryPattern BinSub STR ''az'' STR ''bz'') && noop && noop) &&
-      STR ''bz'' == STR ''b'' && check Empty) ?
+      STR ''bz'' == STR ''b'' && condition Empty) ?
         base (VariableExpr STR ''az'' VoidStamp)"
   by eval
 
 corollary
   "AddLeftNegateToSub =
    (MATCH.match STR ''e'' (BinaryPattern BinAdd STR ''a'' STR ''b'') && noop &&
-    (MATCH.match STR ''b'' (UnaryPattern UnaryNeg STR ''az'') && noop) && check Empty) ?
+    (MATCH.match STR ''b'' (UnaryPattern UnaryNeg STR ''az'') && noop) && condition Empty) ?
       base (BinaryExpr BinSub 
             (VariableExpr STR ''a'' VoidStamp)
             (VariableExpr STR ''az'' VoidStamp))"
@@ -1231,12 +2632,12 @@ corollary
    (MATCH.match STR ''a'' (BinaryPattern BinSub STR ''az'' STR ''bz'') ?
     (noop ?
      (noop ?
-      (STR ''bz'' == STR ''b'' ? (check Empty ? base (VariableExpr STR ''az'' VoidStamp)))))) else
+      (STR ''bz'' == STR ''b'' ? (condition Empty ? base (VariableExpr STR ''az'' VoidStamp)))))) else
    MATCH.match STR ''e'' (BinaryPattern BinAdd STR ''a'' STR ''b'') ?
    (noop ?
     (MATCH.match STR ''b'' (UnaryPattern UnaryNeg STR ''az'') ?
      (noop ?
-      (check Empty ?
+      (condition Empty ?
        base
         (BinaryExpr BinSub (VariableExpr STR ''a'' VoidStamp)
           (VariableExpr STR ''az'' VoidStamp)))))))"
@@ -1247,16 +2648,17 @@ corollary
    (MATCH.match STR ''e'' (BinaryPattern BinAdd STR ''a'' STR ''b'') ?
    (MATCH.match STR ''a'' (BinaryPattern BinSub STR ''az'' STR ''bz'') ?
     (noop ?
-     (STR ''bz'' == STR ''b'' ? (check Empty ? base (VariableExpr STR ''az'' VoidStamp)))) else
+     (STR ''bz'' == STR ''b'' ? (condition Empty ? base (VariableExpr STR ''az'' VoidStamp)))) else
     noop ?
     (MATCH.match STR ''b'' (UnaryPattern UnaryNeg STR ''az'') ?
      (noop ?
-      (check Empty ?
+      (condition Empty ?
        base
         (BinaryExpr BinSub (VariableExpr STR ''a'' VoidStamp)
           (VariableExpr STR ''az'' VoidStamp)))))))"
   by eval
 
+(* lift_common removed from optimized export 
 corollary
   "optimized_export (RedundantSub else AddLeftNegateToSub) =
    MATCH.match STR ''e'' (BinaryPattern BinAdd STR ''a'' STR ''b'') ?
@@ -1266,13 +2668,15 @@ corollary
     else
     MATCH.match STR ''b'' (UnaryPattern UnaryNeg STR ''az'') ?
      base (BinaryExpr BinSub (VariableExpr STR ''a'' VoidStamp) (VariableExpr STR ''az'' VoidStamp)))"
-  by eval
+  by eval*)
 
 subsubsection \<open>Java Generation\<close>
 
-value "export_rules RedundantSub"
+value "RedundantSub"
+value "(export_rules RedundantSub)"
+value "generate_statement 0 (export_rules RedundantSub)"
 value "export_rules AddLeftNegateToSub"
-value "export_rules (RedundantSub else AddLeftNegateToSub)"
+value "generate_statement 0 (export_rules (RedundantSub else AddLeftNegateToSub))"
 
 value "export_rules (lift_common (lift_match (RedundantSub else AddLeftNegateToSub)))"
 value "export_rules (optimized_export (RedundantSub else AddLeftNegateToSub))"
@@ -1282,10 +2686,64 @@ value "export_rules (optimized_export ((RedundantSub else AddLeftNegateToSub) el
 value "export_rules (optimized_export (NestedNot else RedundantSub else AddLeftNegateToSub))"
 
 no_notation cond (infixl "?" 52)
-no_notation seq (infixl "&&" 50)
+no_notation seq (infixl "\<then>" 50)
+no_notation andthen (infixl "&&" 50)
 
-notation And (infixl "&&" 50)
+notation SideCondition.And (infixl "&&" 50)
 
 value "NestedNot \<then> (RedundantSub else AddLeftNegateToSub)"
+
+
+subsection \<open>Examples\<close>
+
+text \<open>@{text "x * const 1 \<longrightarrow> x"}\<close>
+definition Identity where
+  "Identity = generate 
+    (BinaryExpr BinMul
+      (var ''x'')
+      (ConstantExpr (IntVal 32 1)))
+    (var ''x'')
+    (Empty)"
+
+value "Identity"
+value "export_rules (optimized_export (Identity))"
+
+text \<open>@{text "const x * const y \<longrightarrow> const (x * y)"}\<close>
+definition Evaluate where
+  "Evaluate = generate 
+    (BinaryExpr BinMul
+      (ConstantVar STR ''x'')
+      (ConstantVar STR ''y''))
+    (ConstantVar STR ''x'')
+    (Empty)"
+(* doesn't support constant evaluation *)
+value "Evaluate"
+value "export_rules (optimized_export (Evaluate))"
+
+text \<open>@{text "x * const y \<longrightarrow> x << const (log2 y)"}\<close>
+definition Shift where
+  "Shift = generate 
+    (BinaryExpr BinMul
+      (var ''x'')
+      (ConstantVar STR ''y''))
+    (BinaryExpr BinLeftShift (var ''x'') (ConstantVar STR ''y''))
+    (PowerOf2 (ConstantVar STR ''y''))"
+(* doesn't support constant evaluation *)
+value "Shift"
+
+
+text \<open>@{text "const x * y \<longrightarrow> y * const x when NotConst y"}\<close>
+definition LeftConst where
+  "LeftConst = generate 
+    (BinaryExpr BinMul
+      (ConstantVar STR ''x'')
+      (var ''y''))
+    (BinaryExpr BinMul (var ''y'') (ConstantVar STR ''x''))
+    (Not (IsConstantExpr (var ''y'')))"
+(* doesn't support constant evaluation *)
+value "LeftConst"
+
+
+value "(optimized_export (optimized_export (LeftConst \<then> (Evaluate else (Identity else Shift)))))"
 
 end
